Prove correctness of freshening

compiler/backend/passes/proofs/pure_freshenProofScript.sml
@@ -2,12 +2,1932 @@
    Correctness for freshening of bound variables.
 *)
 open HolKernel Parse boolLib bossLib BasicProvers dep_rewrite;
-open pairTheory listTheory rich_listTheory pred_setTheory
-open pure_expTheory pure_cexpTheory pureLangTheory pure_congruenceTheory
-     pure_varsTheory var_setTheory
-     pure_freshenTheory pure_barendregtTheory;
+open pairTheory listTheory alistTheory rich_listTheory pred_setTheory
+     finite_mapTheory;
+open pure_miscTheory pure_expTheory pure_cexpTheory pureLangTheory
+     pure_alpha_equivTheory pure_congruenceTheory pure_beta_equivTheory
+     pure_barendregtTheory pure_exp_lemmasTheory
+     pure_varsTheory var_setTheory pure_freshenTheory pure_letrecProofTheory;
 
 val _ = new_theory "pure_freshenProof";
+
+
+(****************************** TODO move ******************************)
+
+Theorem boundvars_subst_SUBSET:
+  ∀m e.  boundvars (subst m e) ⊆ boundvars e ∪ BIGUNION (IMAGE boundvars $ FRANGE m)
+Proof
+  recInduct subst_ind >> rw[subst_def]
+  >- (
+    CASE_TAC >> rw[SUBSET_DEF, PULL_EXISTS, IN_FRANGE_FLOOKUP] >>
+    rpt $ goal_assum drule
+    )
+  >- (
+    simp[MAP_MAP_o, combinTheory.o_DEF] >> rw[BIGUNION_SUBSET, MEM_MAP] >>
+    first_x_assum drule >> strip_tac >>
+    irule SUBSET_TRANS >> goal_assum drule >> rw[SUBSET_DEF] >> disj1_tac >>
+    simp[MEM_MAP, PULL_EXISTS, SF SFY_ss]
+    )
+  >- (irule SUBSET_TRANS >> goal_assum drule >> simp[SUBSET_DEF])
+  >- (irule SUBSET_TRANS >> goal_assum drule >> simp[SUBSET_DEF])
+  >- (
+    irule SUBSET_TRANS >> goal_assum drule >>
+    rw[SUBSET_DEF, PULL_EXISTS, IN_FRANGE_FLOOKUP] >>
+    gvs[DOMSUB_FLOOKUP_THM, SF SFY_ss]
+    )
+  >- (
+    irule SUBSET_TRANS >> goal_assum drule >> rw[] >- simp[SUBSET_DEF] >>
+    rw[BIGUNION_SUBSET, SUBSET_DEF, PULL_EXISTS] >> rpt disj2_tac >>
+    gvs[IN_FRANGE_FLOOKUP, PULL_EXISTS, FLOOKUP_SIMP, SF SFY_ss]
+    )
+  >- (
+    simp[MAP_MAP_o, combinTheory.o_DEF, LAMBDA_PROD, GSYM FST_THM] >> rw[SUBSET_DEF]
+    )
+  >- (
+    simp[MAP_MAP_o, combinTheory.o_DEF, LAMBDA_PROD, GSYM FST_THM] >>
+    rw[BIGUNION_SUBSET, MEM_MAP] >> pairarg_tac >> gvs[] >>
+    first_x_assum drule >> rw[] >> irule SUBSET_TRANS >> goal_assum drule >> rw[]
+    >- rw[SUBSET_DEF, PULL_EXISTS, MEM_MAP, EXISTS_PROD, SF SFY_ss] >>
+    rw[BIGUNION_SUBSET, SUBSET_DEF, PULL_EXISTS] >> rpt disj2_tac >>
+    gvs[IN_FRANGE_FLOOKUP, PULL_EXISTS, FLOOKUP_SIMP, SF SFY_ss]
+    )
+QED
+
+Theorem allvars_thm:
+  allvars e = freevars e ∪ boundvars e
+Proof
+  Induct_on `e` using freevars_ind >>
+  rw[allvars_def, freevars_def, boundvars_def]
+  >- (Induct_on `es` >> rw[] >> gvs[] >> rw[Once EXTENSION] >> metis_tac[])
+  >- (rw[EXTENSION] >> metis_tac[])
+  >- (rw[EXTENSION] >> metis_tac[]) >>
+  simp[AC UNION_ASSOC UNION_COMM] >> AP_TERM_TAC >>
+  simp[UNION_ASSOC] >>
+  qmatch_goalsub_abbrev_tac `_ = a ∪ b ∪ (c DIFF _)` >>
+  `a ∪ b ∪ (c DIFF a) = a ∪ b ∪ c` by (rw[EXTENSION] >> metis_tac[]) >>
+  rw[] >> unabbrev_all_tac >>
+  simp[AC UNION_ASSOC UNION_COMM] >> ntac 2 AP_TERM_TAC >>
+  ntac 2 $ pop_assum kall_tac >> Induct_on `lcs` >> rw[] >>
+  pairarg_tac >> gvs[SF DNF_ss] >> last_x_assum drule >> rw[] >>
+  rw[Once EXTENSION] >> metis_tac[]
+QED
+
+Theorem set_MAP_SND_fmap_to_alist:
+  set (MAP SND (fmap_to_alist m)) = FRANGE m
+Proof
+  rw[fmap_to_alist_def, EXTENSION, MEM_MAP, EXISTS_PROD, IN_FRANGE_FLOOKUP]
+QED
+
+Theorem allvars_subst_SUBSET:
+  allvars (subst m e) ⊆ allvars e ∪ BIGUNION (IMAGE allvars (FRANGE m))
+Proof
+  rw[SUBSET_DEF, allvars_thm] >>
+  imp_res_tac $ SRULE [SUBSET_DEF] freevars_subst_SUBSET >>
+  imp_res_tac $ SRULE [SUBSET_DEF] boundvars_subst_SUBSET >>
+  gvs[PULL_EXISTS] >> metis_tac[]
+QED
+
+Theorem ALOOKUP_REVERSE_fmap_to_alist[simp]:
+  ALOOKUP (REVERSE (fmap_to_alist m)) = ALOOKUP (fmap_to_alist m)
+Proof
+  rw[FUN_EQ_THM] >>
+  Cases_on `ALOOKUP (REVERSE (fmap_to_alist m)) x`
+  >- gvs[ALOOKUP_NONE, MAP_REVERSE, FLOOKUP_DEF]
+  >- (imp_res_tac ALOOKUP_MEM >> gvs[])
+QED
+
+Theorem EL_split:
+  ∀l n. n < LENGTH l ⇒ l = TAKE n l ++ [EL n l] ++ DROP (n + 1) l
+Proof
+  rw[] >> qspecl_then [`1`,`n`,`l`] assume_tac TAKE_SEG_DROP >> gvs[SEG1]
+QED
+
+Theorem boundvars_Apps:
+  boundvars (Apps e es) =
+    boundvars e ∪ BIGUNION (set $ MAP boundvars es)
+Proof
+  Induct_on `es` using SNOC_INDUCT >> rw[Apps_def, SNOC_APPEND, Apps_append] >>
+  simp[AC UNION_ASSOC UNION_COMM]
+QED
+
+Theorem FRANGE_FUPDATE_LIST_ALL_DISTINCT:
+  ∀l m.
+    ALL_DISTINCT (MAP FST l) ⇒
+    set (MAP SND l) ⊆ FRANGE (m |++ l)
+Proof
+  Induct_on `l` using SNOC_INDUCT >> rw[] >>
+  gvs[SNOC_APPEND, FUPDATE_LIST_APPEND, ALL_DISTINCT_APPEND] >>
+  PairCases_on `x` >> gvs[FUPDATE_LIST_THM] >>
+  gvs[DOMSUB_FUPDATE_LIST] >>
+  qmatch_goalsub_abbrev_tac `FILTER f l`  >>
+  qsuff_tac `FILTER f l = l` >- gvs[SUBSET_DEF] >>
+  simp[FILTER_EQ_ID] >> unabbrev_all_tac >>
+  gvs[EVERY_MEM, MEM_MAP, combinTheory.o_DEF, FORALL_PROD]
+QED
+
+Theorem boundvars_Disj[simp]:
+  boundvars (Disj x cnars) = {}
+Proof
+  Induct_on `cnars` >> rw[Disj_def] >>
+  PairCases_on `h` >> rw[Disj_def]
+QED
+
+Theorem boundvars_lets_for:
+  boundvars (lets_for cn x projs e) =
+    boundvars e ∪ set (MAP SND projs)
+Proof
+  Induct_on `projs` >> rw[lets_for_def] >>
+  PairCases_on `h` >> rw[lets_for_def] >>
+  rw[EXTENSION] >> metis_tac[]
+QED
+
+Theorem letrecs_distinct_Disj[simp]:
+  letrecs_distinct (Disj x cnars) = T
+Proof
+  Induct_on `cnars` >> rw[Disj_def, letrecs_distinct_def] >>
+  PairCases_on `h` >> rw[Disj_def, letrecs_distinct_def]
+QED
+
+Theorem letrecs_distinct_IfDisj[simp]:
+  letrecs_distinct (IfDisj x cnars e) ⇔
+  letrecs_distinct e
+Proof
+  Induct_on `cnars` >> rw[IfDisj_def, letrecs_distinct_def]
+QED
+
+
+
+(****************************** Relations ******************************)
+
+Overload subst_vars = ``λm. subst (Var o_f m)``;
+Overload subst1_var = ``λx y. subst_vars (FEMPTY |+ (x,y))``;
+
+
+(********** substitution **********)
+
+Inductive freshen_subst:
+  freshen_subst avoid (Var x) (Var x) ∧
+
+  (LIST_REL (freshen_subst avoid) es es'
+    ⇒ freshen_subst avoid (Prim op es) (Prim op es')) ∧
+
+  (y ∉ avoid ∧
+   freshen_subst (y INSERT avoid) (subst1_var x y e) e'
+    ⇒ freshen_subst avoid (Lam x e) (Lam y e')) ∧
+
+  (freshen_subst avoid e1 e1' ∧ freshen_subst avoid e2 e2'
+    ⇒ freshen_subst avoid (App e1 e2) (App e1' e2')) ∧
+
+  (FDOM m = set (MAP FST fns) ∧
+   DISJOINT (FRANGE m) avoid ∧
+   (∀k k' v. FLOOKUP m k = SOME v ∧ FLOOKUP m k' = SOME v ⇒ k = k') ∧
+   LIST_REL (λ(f,body) (f',body').
+      FLOOKUP m f = SOME f' ∧
+      freshen_subst (avoid ∪ FRANGE m)
+        (subst_vars m body) body') fns fns' ∧
+   freshen_subst (avoid ∪ FRANGE m) (subst_vars m e) e'
+    ⇒ freshen_subst avoid (Letrec fns e) (Letrec fns' e'))
+End
+
+Theorem perm_exp_alpha_subst:
+  y ∉ allvars e ⇒
+    exp_alpha (perm_exp x y e) (subst1 x (Var y) e)
+Proof
+  simp[allvars_thm] >>
+  Induct_on `e` using freevars_ind >> rw[perm_exp_def, subst1_def, perm1_simps] >>
+  gvs[exp_alpha_refl]
+  >- rw[perm1_def, exp_alpha_refl]
+  >- (
+    irule exp_alpha_Prim >>
+    gvs[LIST_REL_EL_EQN, EL_MAP, MEM_EL, PULL_EXISTS] >> rw[] >>
+    last_x_assum drule >> disch_then irule >> metis_tac[EL_MAP]
+    )
+  >- (irule exp_alpha_App >> simp[])
+  >- (
+    simp[Once exp_alpha_cases] >>
+    simp[Once perm_exp_compose, perm1_simps] >> disj2_tac >>
+    simp[freevars_eqvt, perm1_def, AllCaseEqs()] >> metis_tac[]
+    )
+  >- (simp[perm1_def] >> irule exp_alpha_Lam >> simp[])
+  >- (
+    irule exp_alpha_sym >>
+    drule exp_alpha_Letrec_Alpha_MEM >> simp[PAIR_MAP_ALT]
+    )
+  >- (
+    irule exp_alpha_Letrec >> rw[MAP_MAP_o, combinTheory.o_DEF, LAMBDA_PROD]
+    >- (
+      rw[MAP_EQ_f] >> pairarg_tac >> gvs[] >>
+      gvs[MEM_MAP, FORALL_PROD] >> rw[perm1_def] >> gvs[]
+      )
+    >- (
+      last_x_assum mp_tac >>
+      rw[LIST_REL_EL_EQN, EL_MAP, MEM_EL, PULL_EXISTS] >>
+      first_x_assum drule >> rpt (pairarg_tac >> gvs[]) >> disch_then irule >>
+      gvs[MEM_MAP, FORALL_PROD] >> metis_tac[EL_MEM]
+      )
+    )
+QED
+
+Theorem perm_exp_list_alpha_subst:
+  ∀binds m e.
+  DISJOINT (FRANGE m) (allvars e) ∧
+  binds_ok binds ∧
+  ALL_DISTINCT (MAP FST binds) ∧
+  set (MAP FST binds) = FDOM m ∧
+  (∀k v. FLOOKUP m k = SOME v ⇒ ALOOKUP binds k = SOME v)
+  ⇒ exp_alpha (perm_exp_list binds e) (subst_vars m e)
+Proof
+  Induct >> rw[] >> gvs[perm_exp_list_def]
+  >- (Cases_on `m` >> gvs[exp_alpha_refl]) >>
+  PairCases_on `h` >> rename1 `x,y` >> gvs[perm_exp_list_def] >>
+  gvs[ALOOKUP_APPEND, AllCaseEqs(), ALOOKUP_NONE, MAP_REVERSE] >>
+  `FLOOKUP m x = SOME y` by (
+    Cases_on `FLOOKUP m x` >> gvs[]
+    >- (gvs[FLOOKUP_DEF, EXTENSION] >> metis_tac[]) >>
+    first_x_assum drule >> rw[] >> gvs[] >>
+    imp_res_tac ALOOKUP_MEM >> gvs[MEM_MAP]) >>
+  `m = m |+ (x,y)` by (irule $ GSYM FUPDATE_ELIM >> gvs[FLOOKUP_DEF]) >>
+  pop_assum SUBST1_TAC >>
+  rewrite_tac[Once FUPDATE_PURGE] >>
+  simp[Once FUPDATE_EQ_FUNION] >> simp[Once FUNION_COMM] >>
+  DEP_REWRITE_TAC[GSYM subst_subst_DISJOINT_FUNION] >> conj_tac
+  >- (
+    simp[GSYM IMAGE_FRANGE, PULL_EXISTS] >>
+    rw[IN_FRANGE_FLOOKUP, DOMSUB_FLOOKUP_THM] >>
+    first_x_assum drule >> rw[] >> gvs[binds_ok_def] >>
+    first_x_assum $ qspec_then `[]` assume_tac >> gvs[] >>
+    imp_res_tac ALOOKUP_MEM >> gvs[MEM_MAP]
+    ) >>
+  irule exp_alpha_Trans >>
+  irule_at Any exp_alpha_perm_closed >>
+  irule_at Any perm_exp_alpha_subst >> rw[]
+  >- (
+    gvs[DISJOINT_ALT, IN_FRANGE_FLOOKUP, PULL_EXISTS] >>
+    CCONTR_TAC >> gvs[] >>
+    drule $ SRULE [SUBSET_DEF] allvars_subst_SUBSET >>
+    strip_tac >> gvs[] >- res_tac >>
+    gvs[IN_FRANGE_FLOOKUP, FLOOKUP_o_f, AllCaseEqs(), DOMSUB_FLOOKUP_THM] >>
+    first_assum drule >> strip_tac >> imp_res_tac ALOOKUP_MEM >>
+    gvs[binds_ok_def] >>
+    qpat_x_assum `∀l x y r. _` $ qspec_then `[]` assume_tac >> gvs[MEM_MAP]
+    ) >>
+  last_x_assum irule >> rw[]
+  >- (gvs[DOMSUB_FLOOKUP_THM] >> first_x_assum drule >> rw[])
+  >- gvs[binds_ok_def]
+  >- (gvs[EXTENSION] >> metis_tac[])
+  >- (
+    gvs[DISJOINT_ALT, IN_FRANGE_FLOOKUP, PULL_EXISTS, DOMSUB_FLOOKUP_THM] >>
+    metis_tac[]
+    )
+QED
+
+Theorem fmap_to_alist_binds_ok:
+  (∀k k' v. FLOOKUP m k = SOME v ∧ FLOOKUP m k' = SOME v ⇒ k = k') ∧
+  DISJOINT (FDOM m) (FRANGE m)
+  ⇒ binds_ok (fmap_to_alist m)
+Proof
+  rw[binds_ok_def]
+  >- (
+    CCONTR_TAC >> gvs[MEM_MAP, EXISTS_PROD] >>
+    `x ∈ FDOM m` by (
+      rewrite_tac[GSYM set_MAP_FST_fmap_to_alist] >>
+      simp[Excl "set_MAP_FST_fmap_to_alist"]) >>
+    `x ∈ FRANGE m` by (
+      simp[GSYM set_MAP_SND_fmap_to_alist, MEM_MAP, EXISTS_PROD, SF SFY_ss]) >>
+    gvs[DISJOINT_ALT]
+    )
+  >- (
+    CCONTR_TAC >> gvs[MEM_MAP, EXISTS_PROD] >>
+    `MEM (x,y) (fmap_to_alist m) ∧ MEM (p_1,y) (fmap_to_alist m)` by (
+      qpat_x_assum `fmap_to_alist _ = _` SUBST_ALL_TAC >> simp[]) >>
+    gvs[] >> first_x_assum dxrule_all >> rw[] >>
+    qspec_then `m` assume_tac ALL_DISTINCT_fmap_to_alist_keys >>
+    qpat_x_assum `fmap_to_alist _ = _` SUBST_ALL_TAC >> simp[] >>
+    gvs[ALL_DISTINCT_APPEND, MEM_MAP, EXISTS_PROD] >> metis_tac[]
+    )
+QED
+
+Theorem freshen_subst_exp_alpha:
+  ∀avoid e1 e2.
+    freshen_subst avoid e1 e2 ∧ allvars e1 ⊆ avoid
+  ⇒ exp_alpha e1 e2
+Proof
+  Induct_on `freshen_subst` >> rw[exp_alpha_refl]
+  >- ( (* Prim *)
+    irule exp_alpha_Prim >> gvs[LIST_REL_EL_EQN] >> rw[] >>
+    first_x_assum drule >> strip_tac >>
+    first_x_assum irule >> gvs[BIGUNION_SUBSET, MEM_MAP, MEM_EL, PULL_EXISTS]
+    )
+  >- ( (* Lam *)
+    `x ≠ y` by (CCONTR_TAC >> gvs[]) >>
+    irule exp_alpha_Trans >> qexists `Lam y (subst1 x (Var y) e)` >>
+    irule_at Any exp_alpha_Trans >> qexists `Lam y (perm_exp x y e)` >>
+    irule_at Any exp_alpha_Lam >> irule_at Any perm_exp_alpha_subst >>
+    irule_at Any exp_alpha_Alpha >>
+    irule_at Any exp_alpha_Lam >> gvs[] >>
+    first_x_assum $ irule_at Any >>
+    irule_at Any SUBSET_TRANS >> irule_at Any allvars_subst_SUBSET >>
+    simp[IN_FRANGE_FLOOKUP, FLOOKUP_SIMP] >>
+    gvs[SUBSET_DEF, allvars_thm] >> metis_tac[]
+    )
+  >- (irule exp_alpha_App >> gvs[]) (* App *) >>
+  (* Letrec *)
+  qpat_x_assum `_ ⇒ exp_alpha _ _` mp_tac >> impl_keep_tac
+  >- (
+    irule SUBSET_TRANS >> irule_at Any allvars_subst_SUBSET >>
+    gvs[SUBSET_DEF, PULL_EXISTS, IN_FRANGE_FLOOKUP, FLOOKUP_o_f, AllCaseEqs()]
+    ) >>
+  strip_tac >> irule exp_alpha_Trans >>
+  irule_at Any exp_alpha_perm_exp_list >>
+  simp[perm_exp_list_Letrec] >>
+  irule_at Any exp_alpha_Letrec >>
+  simp[MAP_MAP_o, combinTheory.o_DEF, LAMBDA_PROD] >>
+  qexists `fmap_to_alist m` >> rw[]
+  >- (
+    irule exp_alpha_Trans >> goal_assum $ drule_at Any >>
+    irule perm_exp_list_alpha_subst >> simp[] >>
+    irule_at Any fmap_to_alist_binds_ok >> simp[] >>
+    gvs[DISJOINT_ALT, SUBSET_DEF, allvars_thm] >> metis_tac[]
+    )
+  >- (
+    rw[MAP_EQ_EVERY2] >> gvs[LIST_REL_EL_EQN] >> rw[] >>
+    first_x_assum drule >> rpt (pairarg_tac >> gvs[]) >> rw[] >>
+    `binds_ok (fmap_to_alist m)` by (
+      irule_at Any fmap_to_alist_binds_ok >> simp[] >>
+      gvs[DISJOINT_ALT, SUBSET_DEF, allvars_thm] >> metis_tac[]) >>
+    drule_at Any perm1_list_apply >> simp[] >>
+    disch_then $ qspec_then `f` mp_tac >>
+    simp[MEM_EL, PULL_EXISTS] >> disch_then drule >> simp[EL_MAP]
+    )
+  >- (
+    gvs[LIST_REL_EL_EQN, EL_MAP] >> rw[] >>
+    first_x_assum drule >> rpt (pairarg_tac >> gvs[]) >> rw[] >>
+    irule exp_alpha_Trans >> first_x_assum $ irule_at Any >>
+    irule_at Any perm_exp_list_alpha_subst >> simp[] >>
+    irule_at Any fmap_to_alist_binds_ok >> simp[] >>
+    irule_at Any SUBSET_TRANS >> irule_at Any allvars_subst_SUBSET >>
+    gvs[DISJOINT_ALT, SUBSET_DEF, allvars_thm,
+        MEM_MAP, MEM_EL, EXISTS_PROD, GSYM IMAGE_FRANGE, PULL_EXISTS] >>
+    metis_tac[]
+    )
+  >- simp[DISJOINT_ALT]
+  >- (
+    simp[set_MAP_SND_fmap_to_alist] >>
+    irule DISJOINT_SUBSET >> goal_assum drule >>
+    gvs[allvars_thm, SUBSET_DEF, MEM_MAP, EXISTS_PROD, PULL_EXISTS] >>
+    metis_tac[]
+    )
+QED
+
+
+(********** stacked substitution **********)
+
+Inductive freshen_stack:
+  (FLOOKUP m x = NONE
+    ⇒ freshen_stack avoid m (Var x) (Var x)) ∧
+
+  (FLOOKUP m x = SOME y
+    ⇒ freshen_stack avoid m (Var x) (Var y)) ∧
+
+  (LIST_REL (freshen_stack avoid m) es es'
+    ⇒ freshen_stack avoid m (Prim op es) (Prim op es')) ∧
+
+  (y ∉ avoid ∧ freshen_stack (y INSERT avoid) (m |+ (x,y)) e e'
+    ⇒ freshen_stack avoid m (Lam x e) (Lam y e')) ∧
+
+  (freshen_stack avoid m e1 e1' ∧ freshen_stack avoid m e2 e2'
+    ⇒ freshen_stack avoid m (App e1 e2) (App e1' e2')) ∧
+
+  (FDOM new = set (MAP FST fns) ∧
+   DISJOINT (FRANGE new) avoid ∧
+   (∀k k' v. FLOOKUP new k = SOME v ∧ FLOOKUP new k' = SOME v ⇒ k = k') ∧
+   LIST_REL (λ(f,body) (f',body').
+      FLOOKUP new f = SOME f' ∧
+      freshen_stack (avoid ∪ FRANGE new) (FUNION new m) body body') fns fns' ∧
+   freshen_stack (avoid ∪ FRANGE new) (FUNION new m) e e'
+   ⇒ freshen_stack avoid m (Letrec fns e) (Letrec fns' e'))
+End
+
+Theorem freshen_stack_freshen_subst:
+  ∀m e1 e2 avoid.
+    freshen_stack avoid m e1 e2 ∧
+    boundvars e1 ⊆ avoid ∧
+    FRANGE m ⊆ avoid ∧
+    DISJOINT (FRANGE m) (boundvars e1)
+  ⇒ freshen_subst avoid (subst_vars m e1) e2
+Proof
+  Induct_on `freshen_stack` >> rw[] >>
+  simp[Once freshen_subst_cases] >> gvs[subst_def, FLOOKUP_o_f]
+  >- (
+    gvs[LIST_REL_EL_EQN, EL_MAP] >> rw[] >>
+    first_x_assum drule >> strip_tac >> pop_assum irule >>
+    gvs[BIGUNION_SUBSET, MEM_MAP, PULL_EXISTS, MEM_EL]
+    )
+  >- (
+    qpat_x_assum `_ ⇒ _` mp_tac >> impl_tac
+    >-  (
+      gvs[SUBSET_DEF, DISJOINT_ALT, IN_FRANGE_FLOOKUP, DOMSUB_FLOOKUP_THM] >>
+      metis_tac[]
+      ) >>
+    strip_tac >>
+    qsuff_tac `subst (Var o_f m |+ (x,Var y)) e1 =
+               subst1 x (Var y) (subst_vars (m \\ x) e1)` >>
+    rw[] >> gvs[] >>
+    rewrite_tac[Once FUPDATE_PURGE, Once FUPDATE_EQ_FUNION] >>
+    DEP_ONCE_REWRITE_TAC[FUNION_COMM] >> simp[] >>
+    DEP_REWRITE_TAC[GSYM subst_subst_DISJOINT_FUNION] >> simp[] >>
+    gvs[IN_FRANGE_FLOOKUP, PULL_EXISTS, FLOOKUP_o_f,
+        DOMSUB_FLOOKUP_THM, AllCaseEqs()]
+    )
+  >- (
+    rpt $ first_x_assum $ irule_at Any >> gvs[DISJOINT_ALT] >> metis_tac[]
+    )
+  >- (
+    gvs[MAP_MAP_o, combinTheory.o_DEF, LAMBDA_PROD] >> gvs[GSYM FST_THM] >>
+    goal_assum drule >> reverse $ rw[]
+    >- (
+      `subst_vars new (subst (FDIFF (Var o_f m) (set (MAP FST fns))) e1) =
+       subst_vars (FUNION new m) e1` by (
+        simp[o_f_FUNION] >> once_rewrite_tac[FUNION_FDIFF] >>
+        DEP_ONCE_REWRITE_TAC[FUNION_COMM] >>
+        DEP_REWRITE_TAC[GSYM subst_subst_DISJOINT_FUNION] >>
+        gvs[FDOM_FDIFF_alt, PULL_EXISTS, IN_FRANGE_FLOOKUP, FLOOKUP_FDIFF,
+            FLOOKUP_o_f, AllCaseEqs(), DISJOINT_ALT] >> metis_tac[]) >>
+      simp[] >> first_x_assum irule >> rw[]
+      >- (
+        irule $ iffLR DISJOINT_SYM >> irule DISJOINT_SUBSET >>
+        irule_at Any FRANGE_FUNION_SUBSET >> simp[] >>
+        gvs[DISJOINT_ALT, SUBSET_DEF] >> metis_tac[]
+        )
+      >- (
+        irule SUBSET_TRANS >> irule_at Any FRANGE_FUNION_SUBSET >> simp[] >>
+        gvs[SUBSET_DEF]
+        )
+      >- gvs[SUBSET_DEF]
+      ) >>
+    gvs[LIST_REL_EL_EQN, EL_MAP] >> rw[] >>
+    first_x_assum drule >> rpt (pairarg_tac >> gvs[]) >>
+    strip_tac >> gvs[] >>
+    `subst_vars new (subst (FDIFF (Var o_f m) (set (MAP FST fns))) e1') =
+     subst_vars (FUNION new m) e1'` by (
+      simp[o_f_FUNION] >> once_rewrite_tac[FUNION_FDIFF] >>
+      DEP_ONCE_REWRITE_TAC[FUNION_COMM] >>
+      DEP_REWRITE_TAC[GSYM subst_subst_DISJOINT_FUNION] >>
+      gvs[FDOM_FDIFF_alt, PULL_EXISTS, IN_FRANGE_FLOOKUP, FLOOKUP_FDIFF,
+          FLOOKUP_o_f, AllCaseEqs(), DISJOINT_ALT] >> metis_tac[]) >>
+    simp[] >> qpat_x_assum `_ ⇒ _` mp_tac >> impl_tac >> rw[]
+    >- (
+      qpat_x_assum `BIGUNION _ ⊆ _` mp_tac >>
+      simp[BIGUNION_SUBSET, MEM_MAP, MEM_EL, PULL_EXISTS] >>
+      disch_then drule >> rw[SUBSET_DEF]
+      )
+    >- (
+      irule SUBSET_TRANS >> irule_at Any FRANGE_FUNION_SUBSET >> simp[] >>
+      gvs[SUBSET_DEF]
+      )
+    >- (
+      irule $ iffLR DISJOINT_SYM >> irule DISJOINT_SUBSET >>
+      irule_at Any FRANGE_FUNION_SUBSET >> simp[] >>
+      gvs[BIGUNION_SUBSET, MEM_MAP, MEM_EL, PULL_EXISTS] >>
+      rpt $ first_x_assum drule >> simp[] >>
+      gvs[DISJOINT_ALT, SUBSET_DEF] >> metis_tac[]
+      )
+    )
+QED
+
+Theorem freshen_stack_mono:
+  ∀avoid m e1 e2 avoid'.
+    freshen_stack avoid m e1 e2 ∧
+    avoid' ⊆ avoid
+  ⇒ freshen_stack avoid' m e1 e2
+Proof
+  Induct_on `freshen_stack` >> rw[] >>
+  simp[Once freshen_stack_cases]
+  >- gvs[LIST_REL_EL_EQN]
+  >- (first_x_assum $ irule_at Any >> gvs[SUBSET_DEF] >> metis_tac[])
+  >- (
+    goal_assum drule >> gvs[] >>
+    irule_at Any DISJOINT_SUBSET >> goal_assum drule >> simp[] >>
+    first_x_assum $ irule_at Any >> rw[] >- gvs[SUBSET_DEF] >>
+    gvs[LIST_REL_EL_EQN] >> rw[] >>
+    first_x_assum drule >> rpt (pairarg_tac >> gvs[]) >> strip_tac >>
+    pop_assum irule >> gvs[SUBSET_DEF]
+    )
+QED
+
+Theorem freshen_stack_boundvars:
+  ∀avoid m e1 e2.
+    freshen_stack avoid m e1 e2 ⇒ DISJOINT (boundvars e2) avoid
+Proof
+  Induct_on `freshen_stack` >> rw[]
+  >- (
+    pop_assum mp_tac >> simp[MEM_MAP, MEM_EL] >> rw[] >> gvs[] >>
+    gvs[LIST_REL_EL_EQN]
+    )
+  >- simp[Once DISJOINT_SYM]
+  >- (
+    rw[DISJOINT_ALT, MEM_MAP, MEM_EL, EXISTS_PROD] >>
+    pop_assum $ assume_tac o GSYM >> gvs[LIST_REL_EL_EQN] >>
+    first_x_assum drule >> rpt (pairarg_tac >> gvs[]) >> rw[] >>
+    `MEM f (MAP FST fns)` by (
+      simp[MEM_MAP, MEM_EL, EXISTS_PROD] >> goal_assum drule >> simp[]) >>
+    qpat_x_assum `FLOOKUP _ _ = _` mp_tac >>
+    simp[FLOOKUP_SIMP, Once FLOOKUP_DEF] >>
+    gvs[FRANGE_DEF, DISJOINT_ALT] >> metis_tac[]
+    )
+  >- (
+    gvs[MEM_MAP, MEM_EL, LIST_REL_EL_EQN] >>
+    first_x_assum drule >> rpt (pairarg_tac >> gvs[]) >> rw[] >>
+    simp[Once DISJOINT_SYM]
+    )
+QED
+
+
+(********** global stacked substitution **********)
+
+Inductive freshen_global:
+  (FLOOKUP m x = NONE
+    ⇒ freshen_global avoid m (Var x) (Var x)) ∧
+
+  (FLOOKUP m x = SOME y
+    ⇒ freshen_global avoid m (Var x) (Var y)) ∧
+
+  (LENGTH es' = LENGTH es ∧
+   (∀l e r. es = l ++ [e] ++ r ⇒
+      ∃l' e' r'. es' = l' ++ [e'] ++ r' ∧ LENGTH l' = LENGTH l ∧
+        freshen_global (avoid ∪ BIGUNION (set (MAP boundvars l'))) m e e')
+    ⇒ freshen_global avoid m (Prim op es) (Prim op es')) ∧
+
+  (y ∉ avoid ∧ freshen_global (y INSERT avoid) (m |+ (x,y)) e e'
+    ⇒ freshen_global avoid m (Lam x e) (Lam y e')) ∧
+
+  (freshen_global avoid m e1 e1' ∧
+   freshen_global (avoid ∪ boundvars e1') m e2 e2'
+    ⇒ freshen_global avoid m (App e1 e2) (App e1' e2')) ∧
+
+  (freshen_global avoid m e1 e1' ∧
+   y ∉ avoid ∪ boundvars e1' ∧
+   freshen_global (y INSERT avoid ∪ boundvars e1') (m |+ (x,y)) e2 e2'
+    ⇒ freshen_global avoid m (Let x e1 e2) (Let y e1' e2')) ∧
+
+  (FDOM new = set (MAP FST fns) ∧
+   DISJOINT (FRANGE new) avoid ∧
+   (∀k k' v. FLOOKUP new k = SOME v ∧ FLOOKUP new k' = SOME v ⇒ k = k') ∧
+   LENGTH fns' = LENGTH fns ∧
+   (∀l f e r. fns = l ++ [f,e] ++ r ⇒
+      ∃l' f' e' r'. fns' = l' ++ [f',e'] ++ r' ∧ LENGTH l' = LENGTH l ∧
+        FLOOKUP new f = SOME f' ∧
+        freshen_global
+          (avoid ∪ FRANGE new ∪ BIGUNION (set $ MAP (λ(f,e). boundvars e) l'))
+          (FUNION new m) e e') ∧
+    freshen_global
+      (avoid ∪ FRANGE new ∪ BIGUNION (set $ MAP (λ(f,e). boundvars e) fns'))
+      (FUNION new m) e e'
+   ⇒ freshen_global avoid m (Letrec fns e) (Letrec fns' e'))
+End
+
+Theorem freshen_global_freshen_stack:
+  ∀m avoid e1 e2.
+    freshen_global avoid m e1 e2 ⇒ freshen_stack avoid m e1 e2
+Proof
+  Induct_on `freshen_global` >> rw[] >>
+  simp[Once freshen_stack_cases]
+  >- (
+    rw[LIST_REL_EL_EQN] >>
+    drule EL_split >> strip_tac >>
+    first_x_assum drule >> rw[] >> gvs[EL_APPEND_EQN] >>
+    irule freshen_stack_mono >> goal_assum $ drule_at Any >> simp[]
+    )
+  >- (irule freshen_stack_mono >> goal_assum $ drule_at Any >> simp[])
+  >- (
+    simp[Once freshen_stack_cases] >>
+    irule freshen_stack_mono >> goal_assum $ drule_at Any >> simp[]
+    )
+  >- (
+    goal_assum drule >> simp[] >>
+    irule_at Any freshen_stack_mono >> goal_assum $ drule_at Any >>
+    conj_tac >- gvs[SUBSET_DEF] >>
+    rw[LIST_REL_EL_EQN] >> rpt (pairarg_tac >> gvs[]) >>
+    drule EL_split >> strip_tac >> gvs[] >>
+    last_x_assum drule >> strip_tac >> gvs[EL_APPEND_EQN] >>
+    irule freshen_stack_mono >> goal_assum $ drule_at Any >> simp[SUBSET_DEF]
+    )
+QED
+
+Theorem freshen_global_boundvars:
+  ∀m avoid e1 e2.
+    freshen_global avoid m e1 e2 ⇒ DISJOINT (boundvars e2) avoid
+Proof
+  rw[] >> dxrule freshen_global_freshen_stack >> rw[] >>
+  dxrule freshen_stack_boundvars >> simp[]
+QED
+
+Theorem freshen_global_mono:
+  ∀m avoid e1 e2 avoid'.
+    freshen_global avoid m e1 e2 ∧ avoid' ⊆ avoid
+  ⇒ freshen_global avoid' m e1 e2
+Proof
+  Induct_on `freshen_global` >> rw[] >> simp[Once freshen_global_cases] >>
+  rw[] >> gvs[]
+  >- (
+    last_x_assum $ qspec_then `l` mp_tac >> rw[] >> gvs[] >>
+    irule_at Any EQ_REFL >> simp[] >>
+    first_x_assum irule >> gvs[SUBSET_DEF]
+    )
+  >- (gvs[SUBSET_DEF] >> CCONTR_TAC >> gvs[])
+  >- ( first_x_assum irule >> gvs[SUBSET_DEF])
+  >- (disj1_tac >> first_x_assum irule >> gvs[SUBSET_DEF])
+  >- (
+    disj2_tac >> first_x_assum $ irule_at Any >> gvs[SUBSET_DEF] >>
+    CCONTR_TAC >> gvs[]
+    )
+  >- (
+    goal_assum drule >> gvs[] >> rw[]
+    >- (irule DISJOINT_SUBSET >> goal_assum drule >> simp[])
+    >- (
+      last_x_assum $ qspec_then `l` mp_tac >> rw[] >>
+      irule_at Any EQ_REFL >> gvs[] >>
+      first_x_assum irule >> gvs[SUBSET_DEF]
+      )
+    >- (first_x_assum irule >> gvs[SUBSET_DEF])
+    )
+QED
+
+(*
+  TODO:
+    letrec_distinct should not be necessary here,
+    if the freshening relations are strengthened
+*)
+Theorem freshen_global_unique_boundvars:
+  ∀m avoid e1 e2.
+    freshen_global avoid m e1 e2 ∧ letrecs_distinct e1
+  ⇒ unique_boundvars e2
+Proof
+  Induct_on `freshen_global` >>
+  rw[unique_boundvars_def, letrecs_distinct_def, list_disjoint_cons] >>
+  gvs[]
+  >- (
+    gvs[EVERY_EL] >> rw[] >> drule EL_split >> strip_tac >>
+    last_x_assum drule >> rw[] >> gvs[EL_APPEND_EQN]
+    )
+  >- (
+    simp[list_disjoint_def, MAP_EQ_APPEND] >> rw[] >> gvs[]
+    >- (
+      rename1 `l' ++ [e'] ++ r'` >> gvs[MEM_MAP, MEM_EL] >>
+      qspecl_then [`es`,`LENGTH l'`] mp_tac EL_split >>
+      simp[] >> strip_tac >>
+      first_x_assum drule >> rw[] >> gvs[EVERY_EL, APPEND_11_LENGTH] >>
+      dxrule freshen_global_boundvars >> rw[DISJOINT_ALT] >>
+      gvs[MEM_MAP, MEM_EL, PULL_EXISTS] >> metis_tac[]
+      )
+    >- (
+      rename1 `l' ++ [e'] ++ r'` >> gvs[MEM_MAP, MEM_EL] >>
+      qspecl_then [`es`,`LENGTH l' + n + 1`] mp_tac EL_split >>
+      simp[] >> strip_tac >>
+      first_x_assum drule >> rw[] >>
+      gvs[APPEND_EQ_APPEND_MID, EL_APPEND_EQN, EVERY_EL] >>
+      rename1 `LENGTH _ + (LENGTH ll + _)` >>
+      `n = LENGTH ll` by DECIDE_TAC >> pop_assum SUBST_ALL_TAC >> gvs[] >>
+      dxrule freshen_global_boundvars >> rw[DISJOINT_ALT]
+      )
+    )
+  >- (dxrule freshen_global_boundvars >> rw[DISJOINT_ALT])
+  >- (dxrule freshen_global_boundvars >> rw[DISJOINT_ALT])
+  >- (dxrule freshen_global_boundvars >> rw[DISJOINT_ALT])
+  >- (dxrule freshen_global_boundvars >> rw[DISJOINT_ALT] >> metis_tac[])
+  >- (
+    `MAP FST fns' = MAP (λx. THE (FLOOKUP new x)) (MAP FST fns)` by (
+      rw[MAP_EQ_EVERY2, LIST_REL_EL_EQN, EL_MAP] >>
+      drule EL_split >> strip_tac >> Cases_on `EL n fns` >>
+      first_x_assum drule >> rw[] >> gvs[EL_APPEND_EQN]) >>
+    simp[] >> irule ALL_DISTINCT_MAP_INJ >> rw[] >>
+    last_x_assum $ qspecl_then [`x`,`y`] mp_tac >> gvs[FLOOKUP_DEF]
+    )
+  >- (
+    simp[list_disjoint_def, MAP_EQ_APPEND] >> rw[] >> gvs[MAP_EQ_APPEND]
+    >- (
+      rename1 `l' ++ [e'] ++ r'` >> gvs[MEM_MAP, MEM_EL] >>
+      qspecl_then [`fns`,`LENGTH l'`] mp_tac EL_split >>
+      simp[] >> strip_tac >> Cases_on `EL (LENGTH l') fns` >>
+      first_x_assum drule >> rw[] >> gvs[EVERY_EL, APPEND_11_LENGTH] >>
+      dxrule freshen_global_boundvars >> rw[DISJOINT_ALT] >>
+      gvs[MEM_MAP, MEM_EL, PULL_EXISTS] >>
+      first_x_assum drule >> pairarg_tac >> gvs[] >> metis_tac[]
+      )
+    >- (
+      rename1 `l' ++ [e'] ++ r'` >> gvs[MEM_MAP, MEM_EL] >>
+      qspecl_then [`fns`,`LENGTH l' + n + 1`] mp_tac EL_split >>
+      simp[] >> strip_tac >>
+      Cases_on `EL (n + (LENGTH l' + 1)) fns` >>
+      first_x_assum drule >> rw[] >>
+      gvs[APPEND_EQ_APPEND_MID, EL_APPEND_EQN, EVERY_EL] >>
+      rename1 `LENGTH _ + (LENGTH ll + _)` >>
+      `n = LENGTH ll` by DECIDE_TAC >> pop_assum SUBST_ALL_TAC >> gvs[] >>
+      dxrule freshen_global_boundvars >> rw[DISJOINT_ALT] >>
+      gvs[MEM_MAP, MEM_EL, PULL_EXISTS] >> PairCases_on `e'` >> gvs[]
+      )
+    )
+  >- (
+    dxrule freshen_global_boundvars >> rw[EVERY_MEM, DISJOINT_ALT] >>
+    gvs[MEM_MAP, EXISTS_PROD, PULL_EXISTS] >> metis_tac[]
+    )
+  >- (
+    simp[Once DISJOINT_SYM] >>
+    irule DISJOINT_SUBSET >> qexists `FRANGE new` >>
+    dxrule freshen_global_boundvars >> rw[EVERY_MEM, DISJOINT_ALT]
+    >- metis_tac[] >>
+    rw[SUBSET_DEF] >> gvs[MEM_MAP, MEM_EL] >>
+    drule EL_split >> strip_tac >> Cases_on `EL n fns` >>
+    first_x_assum drule >> rw[] >> gvs[EL_APPEND_EQN] >>
+    gvs[IN_FRANGE_FLOOKUP, SF SFY_ss]
+    )
+  >- (
+    gvs[EVERY_EL, EL_MAP] >> rw[] >>
+    simp[Once DISJOINT_SYM] >> irule DISJOINT_SUBSET >>
+    qexists `FRANGE new` >> rw[]
+    >- (
+      drule EL_split >> strip_tac >> Cases_on `EL n fns` >>
+      rpt $ first_x_assum drule >> rw[] >> gvs[EL_APPEND_EQN] >>
+      dxrule freshen_global_boundvars >> rw[DISJOINT_ALT] >> metis_tac[]
+      )
+    >- (
+      rw[SUBSET_DEF] >> gvs[MEM_MAP, MEM_EL] >>
+      drule EL_split >> strip_tac >> Cases_on `EL n' fns` >>
+      last_x_assum drule >> rw[] >> gvs[EL_APPEND_EQN] >>
+      gvs[IN_FRANGE_FLOOKUP, SF SFY_ss]
+      )
+    )
+  >- (
+    gvs[EVERY_EL] >> rw[] >> drule EL_split >> strip_tac >>
+    first_x_assum drule >> rw[] >> Cases_on `EL n fns` >>
+    last_x_assum drule >> rw[] >> gvs[EL_APPEND_EQN, EL_MAP]
+    )
+QED
+
+Theorem unique_boundvars_letrecs_distinct:
+  ∀e. unique_boundvars e ⇒ letrecs_distinct e
+Proof
+  Induct using unique_boundvars_ind >>
+  rw[unique_boundvars_def, letrecs_distinct_def] >> gvs[EVERY_MEM]
+QED
+
+Theorem freshen_global_Lams:
+  ∀xs ex ys ey avoid m.
+    LENGTH xs = LENGTH ys ∧
+    DISJOINT (set ys) avoid ∧
+    ALL_DISTINCT ys ∧
+    freshen_global (avoid ∪ set ys) (m |++ ZIP (xs,ys)) ex ey
+  ⇒ freshen_global avoid m (Lams xs ex) (Lams ys ey)
+Proof
+  Induct >> rw[Lams_def] >> gvs[FUPDATE_LIST_THM] >>
+  rename1 `x::xs` >> namedCases_on `ys` ["","y ys"] >> gvs[Lams_def] >>
+  simp[Once freshen_global_cases] >> last_x_assum irule >> simp[] >>
+  gvs[FUPDATE_LIST_THM] >>
+  qmatch_goalsub_abbrev_tac `freshen_global A` >>
+  qmatch_asmsub_abbrev_tac `freshen_global B` >>
+  qsuff_tac `A = B` >> gvs[] >>
+  unabbrev_all_tac >> rw[EXTENSION] >> gvs[] >> metis_tac[]
+QED
+
+Theorem freshen_global_Disj:
+  FLOOKUP m x = SOME y ⇒
+  freshen_global avoid m (Disj x cnars) (Disj y cnars)
+Proof
+  Induct_on `cnars` >> rw[Disj_def]
+  >- simp[Once freshen_global_cases] >>
+  PairCases_on `h` >> rw[Disj_def] >>
+  rw[Once freshen_global_cases] >> Cases_on `l` >> gvs[]
+  >- (
+    rw[Once freshen_global_cases] >> Cases_on `l` >> gvs[] >>
+    simp[Once freshen_global_cases]
+    ) >>
+  Cases_on `t` >> gvs[LENGTH_EQ_NUM_compute, PULL_EXISTS]
+  >- simp[Once freshen_global_cases] >>
+  Cases_on `t'` >> gvs[LENGTH_EQ_NUM_compute, PULL_EXISTS]
+QED
+
+Theorem freshen_global_IfDisj:
+  FLOOKUP m (explode x) = SOME (explode y) ∧ freshen_global avoid m e1 e2 ⇒
+  freshen_global avoid m (IfDisj x cnars e1) (IfDisj y cnars e2)
+Proof
+  rw[IfDisj_def] >>
+  rw[Once freshen_global_cases] >> Cases_on `l` >> gvs[]
+  >- (irule freshen_global_Disj >> simp[]) >>
+  Cases_on `t` >> gvs[LENGTH_EQ_NUM_compute, PULL_EXISTS] >>
+  Cases_on `t'` >> gvs[LENGTH_EQ_NUM_compute, PULL_EXISTS] >>
+  simp[Once freshen_global_cases]
+QED
+
+Theorem freshen_global_lets_for:
+  ∀projs1 projs2 x y avoid m e1 e2.
+    ¬MEM x (MAP SND projs1) ∧
+    FLOOKUP m x = SOME y ∧
+    freshen_global (avoid ∪ set (MAP SND projs2))
+      (m |++ ZIP (MAP SND projs1, MAP SND projs2)) e1 e2 ∧
+    MAP FST projs2 = MAP FST projs1 ∧
+    ALL_DISTINCT (MAP SND projs2) ∧
+    DISJOINT (set (MAP SND projs2)) avoid
+  ⇒ freshen_global avoid m (lets_for cn x projs1 e1) (lets_for cn y projs2 e2)
+Proof
+  Induct >> rw[lets_for_def] >> gvs[FUPDATE_LIST_THM] >>
+  PairCases_on `h` >> gvs[] >>
+  Cases_on `projs2` >> gvs[] >> PairCases_on `h` >> gvs[lets_for_def] >>
+  simp[Once freshen_global_cases] >> disj2_tac >> rw[]
+  >- (
+    rw[Once freshen_global_cases] >> Cases_on `l` >> gvs[] >>
+    simp[Once freshen_global_cases]
+    ) >>
+  last_x_assum irule >> simp[] >> gvs[FLOOKUP_SIMP, FUPDATE_LIST_THM] >>
+  qmatch_goalsub_abbrev_tac `freshen_global A` >>
+  qmatch_asmsub_abbrev_tac `freshen_global B` >>
+  qsuff_tac `A = B` >> gvs[] >>
+  unabbrev_all_tac >> rw[EXTENSION] >> metis_tac[]
+QED
+
+Theorem freshen_global_rows_of:
+  ∀css1 css2 x y avoid m k1 k2.
+    FLOOKUP m x = SOME y ∧
+    freshen_global
+      (avoid ∪ BIGUNION (set $ MAP (λ(cn,pvs,ce). set pvs ∪ boundvars ce) css2))
+      m k1 k2 ∧
+    LENGTH css1 = LENGTH css2 ∧
+    (∀l1 cn pvs1 ce1 r1. css1 = l1 ++ [cn,pvs1,ce1] ++ r1 ⇒
+      ¬ MEM x pvs1 ∧
+      ∃l2 pvs2 ce2 r2. css2 = l2 ++ [cn,pvs2,ce2] ++ r2 ∧
+        LENGTH l2 = LENGTH l1 ∧ LENGTH pvs2 = LENGTH pvs1 ∧
+        ALL_DISTINCT pvs2 ∧
+        DISJOINT (set pvs2) avoid ∧
+        EVERY (λ(cn,pvs,ce). DISJOINT (set pvs2) (set pvs ∪ boundvars ce)) l2 ∧
+        freshen_global
+          (avoid ∪ set pvs2 ∪
+           BIGUNION (set $ MAP (λ(cn,pvs,ce). set pvs ∪ boundvars ce) l2))
+          (m |++ ZIP(pvs1,pvs2)) ce1 ce2)
+  ⇒ freshen_global avoid m (rows_of x k1 css1) (rows_of y k2 css2)
+Proof
+  Induct >> rw[rows_of_def] >> gvs[] >>
+  PairCases_on `h` >> Cases_on `css2` >> gvs[] >>
+  PairCases_on `h` >> gvs[rows_of_def] >>
+  first_assum $ qspec_then `[]` mp_tac >>
+  first_x_assum $ qspec_then `(h0,h1,h2)::l1` $ mp_tac o GEN_ALL >> rw[] >>
+  rw[Once freshen_global_cases] >> Cases_on `l` >> gvs[]
+  >- (
+    rw[Once freshen_global_cases] >> Cases_on `l` >> gvs[] >>
+    simp[Once freshen_global_cases]
+    ) >>
+  Cases_on `t'` >> gvs[LENGTH_EQ_NUM_compute, PULL_EXISTS]
+  >- (
+    irule freshen_global_lets_for >>
+    simp[indexedListsTheory.MAP_MAPi, combinTheory.o_DEF, GSYM MAPi_EQ_l]
+    ) >>
+  Cases_on `t''` >> gvs[LENGTH_EQ_NUM_compute, PULL_EXISTS] >>
+  simp[boundvars_lets_for, combinTheory.o_DEF] >>
+  last_x_assum irule >> simp[] >> reverse conj_tac
+  >- (
+    qmatch_goalsub_abbrev_tac `freshen_global A _ k1` >>
+    qmatch_asmsub_abbrev_tac `freshen_global B _ k1` >>
+    qsuff_tac `A = B` >> gvs[] >>
+    unabbrev_all_tac >> rw[EXTENSION] >> metis_tac[]
+    ) >>
+  rw[] >> first_x_assum $ qspec_then `l1` mp_tac >> rw[] >>
+  Cases_on `l2` >> gvs[] >> irule_at Any EQ_REFL >> rw[]
+  >- simp[Once DISJOINT_SYM] >>
+  qmatch_goalsub_abbrev_tac `freshen_global A` >>
+  qmatch_asmsub_abbrev_tac `freshen_global B` >>
+  qsuff_tac `A = B` >> gvs[] >>
+  unabbrev_all_tac >> rw[EXTENSION] >> metis_tac[]
+QED
+
+
+
+(****************************** Implementation ******************************)
+
+(********** simple lemmas **********)
+
+Theorem freshen_return[simp] = freshen_return_def;
+Theorem freshen_bind[simp]:
+  freshen_bind g f = λs. let (r,s') = g s in f r s'
+Proof
+  simp[freshen_bind_def, combinTheory.o_DEF, UNCURRY]
+QED
+
+Triviality freshen_aux_list_LENGTH:
+  ∀l m avoid l' avoid'.
+    freshen_aux_list m l avoid = (l', avoid')
+  ⇒ LENGTH l' = LENGTH l
+Proof
+  Induct >> rw[freshen_aux_def] >>
+  rpt (pairarg_tac >> gvs[]) >>
+  first_x_assum drule >> simp[]
+QED
+
+Theorem freshen_aux_list_append:
+  freshen_aux_list varmap (l1 ++ l2) = do
+    l1' <- freshen_aux_list varmap l1;
+    l2' <- freshen_aux_list varmap l2;
+    return (l1' ++ l2')
+  od
+Proof
+  Induct_on `l1` >> rw[FUN_EQ_THM] >>
+  rpt (pairarg_tac >> gvs[freshen_aux_def])
+QED
+
+Theorem freshen_mapM_LENGTH:
+  ∀l f avoid l' avoid'.
+    freshen_mapM f l avoid = (l', avoid')
+  ⇒ LENGTH l' = LENGTH l
+Proof
+  Induct >> rw[freshen_mapM_def] >>
+  rpt (pairarg_tac >> gvs[]) >> res_tac
+QED
+
+Theorem freshen_mapM_append:
+  freshen_mapM f (l1 ++ l2) = do
+    l1' <- freshen_mapM f l1;
+    l2' <- freshen_mapM f l2;
+    return (l1' ++ l2')
+  od
+Proof
+  Induct_on `l1` >> rw[FUN_EQ_THM, freshen_mapM_def] >>
+  rpt (pairarg_tac >> gvs[])
+QED
+
+Theorem fresh_boundvars_LENGTH:
+  ∀xs varmap avoid ys varmap' avoid'.
+    fresh_boundvars xs varmap avoid = ((ys,varmap'), avoid')
+  ⇒ LENGTH ys = LENGTH xs
+Proof
+  Induct >> rw[fresh_boundvars_def] >>
+  rpt (pairarg_tac >> gvs[]) >> res_tac
+QED
+
+Theorem fresh_boundvars_append:
+  ∀l1 l2 varmap.
+    fresh_boundvars (l1 ++ l2) varmap = do
+      (l1',varmap') <- fresh_boundvars l1 varmap;
+      (l2',varmap'') <- fresh_boundvars l2 varmap';
+      return (l1' ++ l2', varmap'')
+    od
+Proof
+  Induct >> rw[FUN_EQ_THM, fresh_boundvars_def] >>
+  rpt (pairarg_tac >> gvs[])
+QED
+
+
+(********** structural properties / lemmas **********)
+
+Theorem fresh_boundvar_vars:
+  fresh_boundvar x varmap avoid = ((y,varmap'), avoid') ∧
+  vars_ok avoid
+  ⇒ vars_ok avoid' ∧ set_of avoid' = explode y INSERT set_of avoid ∧
+    explode y ∉ set_of avoid
+Proof
+  strip_tac >> gvs[fresh_boundvar_def] >> rpt (pairarg_tac >> gvs[]) >>
+  drule_all invent_var_thm >> strip_tac >> gvs[]
+QED
+
+Theorem fresh_boundvars_vars:
+  ∀xs varmap avoid ys varmap' avoid'.
+    fresh_boundvars xs varmap avoid = ((ys,varmap'), avoid') ∧
+    vars_ok avoid
+  ⇒ vars_ok avoid' ∧
+    set_of avoid' = set (MAP explode ys) ∪ set_of avoid ∧
+    DISJOINT (set (MAP explode ys)) (set_of avoid) ∧
+    ALL_DISTINCT ys
+Proof
+  Induct >> rpt gen_tac >> strip_tac >> gvs[fresh_boundvars_def] >>
+  rpt (pairarg_tac >> gvs[]) >>
+  dxrule_all fresh_boundvar_vars >> strip_tac >>
+  last_x_assum drule_all >> simp[] >> strip_tac >>
+  gvs[MEM_MAP] >> rw[EXTENSION] >> metis_tac[]
+QED
+
+Theorem freshen_aux_mono:
+  (∀varmap (ce1:'a cexp) avoid1 ce2 avoid2.
+    freshen_aux varmap ce1 avoid1 = (ce2,avoid2) ∧ vars_ok avoid1
+    ⇒ vars_ok avoid2 ∧ set_of avoid1 ⊆ set_of avoid2) ∧
+  (∀varmap (ces1:'a cexp list) avoid1 ces2 avoid2.
+    freshen_aux_list varmap ces1 avoid1 = (ces2,avoid2) ∧ vars_ok avoid1
+    ⇒ vars_ok avoid2 ∧ set_of avoid1 ⊆ set_of avoid2)
+Proof
+  ho_match_mp_tac freshen_aux_ind >> simp[freshen_aux_def] >>
+  rpt conj_tac >> rpt gen_tac
+  >- simp[SUBSET_DEF] >>
+  strip_tac >> rpt gen_tac >> strip_tac >>
+  rpt (pairarg_tac >> gvs[]) >>
+  rpt (first_x_assum dxrule_all >> strip_tac) >> gvs[]
+  >- gvs[SUBSET_DEF]
+  >- (
+    dxrule_all fresh_boundvars_vars >> strip_tac >>
+    first_x_assum dxrule_all >> rw[] >> gvs[SUBSET_DEF]
+    )
+  >- (
+    dxrule_all fresh_boundvar_vars >> strip_tac >>
+    first_x_assum dxrule_all >> rw[] >> gvs[SUBSET_DEF]
+    )
+  >- (
+    dxrule_all fresh_boundvars_vars >> strip_tac >>
+    rename1 `freshen_mapM _ _ s1 = (fns',s2)` >>
+    `vars_ok s2 ∧ set_of s1 ⊆ set_of s2` by (
+      map_every (fn p => qpat_x_assum p mp_tac)
+        [`vars_ok _`,`freshen_mapM _ _ _ = _`,`∀f c m. _ ⇒ _`] >>
+      rpt $ pop_assum kall_tac >> map_every qid_spec_tac [`s1`, `fns'`] >>
+      Induct_on `fns` >> rw[freshen_mapM_def] >> gvs[] >>
+      rpt (pairarg_tac >> gvs[]) >> gvs[DISJ_IMP_THM, FORALL_AND_THM] >>
+      rpt (first_x_assum dxrule_all >> strip_tac) >> gvs[SUBSET_DEF]) >>
+    last_x_assum dxrule_all >> rw[] >> gvs[SUBSET_DEF]
+    )
+  >- (
+    dxrule_all fresh_boundvar_vars >> strip_tac >>
+    rename1 `freshen_mapM _ _ s1 = (css',s2)` >>
+    `vars_ok s2 ∧ set_of s1 ⊆ set_of s2` by (
+      map_every (fn p => qpat_x_assum p mp_tac)
+        [`vars_ok _`,`freshen_mapM _ _ _ = _`,`∀cn pvs ce vm. _ ⇒ _`] >>
+      rpt $ pop_assum kall_tac >> map_every qid_spec_tac [`s1`, `css'`] >>
+      Induct_on `css` >> rw[freshen_mapM_def] >> gvs[] >>
+      rpt (pairarg_tac >> gvs[]) >> gvs[DISJ_IMP_THM, FORALL_AND_THM] >>
+      dxrule_all fresh_boundvars_vars >> strip_tac >>
+      rpt (first_x_assum dxrule_all >> strip_tac) >> gvs[SUBSET_DEF]) >>
+    `vars_ok avoid2 ∧ set_of s2 ⊆ set_of avoid2` by (
+      Cases_on `usopt` >> gvs[] >> PairCases_on `x` >> gvs[] >>
+      rpt (pairarg_tac >> gvs[]) >> first_x_assum drule_all >> simp[]) >>
+    gvs[SUBSET_DEF]
+    )
+  >- gvs[SUBSET_DEF]
+QED
+
+Definition avoid_ok_def:
+  avoid_ok avoid ce ⇔
+    vars_ok avoid ∧
+    allvars (exp_of ce) ⊆ set_of avoid
+End
+
+Theorem avoid_ok_simps[simp]:
+  (avoid_ok avoid (Prim c op ces) ⇔ EVERY (avoid_ok avoid) ces ∧ vars_ok avoid) ∧
+  (avoid_ok avoid (Let c x ce1 ce2) ⇔
+    avoid_ok avoid ce1 ∧ avoid_ok avoid ce2 ∧ explode x ∈ set_of avoid) ∧
+  (avoid_ok avoid (Lam c xs ce) ⇔
+    avoid_ok avoid ce ∧ set (MAP explode xs) ⊆ set_of avoid) ∧
+  (avoid_ok avoid (App c ce ces) ⇔ avoid_ok avoid ce ∧ EVERY (avoid_ok avoid) ces) ∧
+  (avoid_ok avoid (Letrec c fns ce) ⇔
+    avoid_ok avoid ce ∧
+    EVERY ( λ(f,ce). avoid_ok avoid ce) fns ∧
+    set (MAP (explode o FST) fns) ⊆ set_of avoid) ∧
+  (avoid_ok avoid (pure_cexp$Case c ce x css usopt) ⇔
+    avoid_ok avoid ce ∧
+    explode x ∈ set_of avoid ∧
+    EVERY (λ(cn,pvs,ce). set (MAP explode pvs) ⊆ set_of avoid ∧ avoid_ok avoid ce) css ∧
+    (∀cnars ce. usopt = SOME (cnars,ce) ⇒ avoid_ok avoid ce))
+Proof
+  rw[avoid_ok_def, exp_of_def, EVERY_MEM, allvars_Apps, allvars_Lams, allvars_rows_of]
+  >- (simp[BIGUNION_SUBSET, MEM_MAP, PULL_EXISTS] >> metis_tac[])
+  >- (simp[BIGUNION_SUBSET, MEM_MAP, PULL_EXISTS] >> metis_tac[])
+  >- (simp[BIGUNION_SUBSET, MEM_MAP, PULL_EXISTS] >> metis_tac[])
+  >- (simp[BIGUNION_SUBSET, MEM_MAP, PULL_EXISTS] >> metis_tac[])
+  >- (
+    gvs[MAP_MAP_o, combinTheory.o_DEF, UNCURRY, FORALL_PROD] >>
+    simp[BIGUNION_SUBSET, MEM_MAP, PULL_EXISTS, EXISTS_PROD] >> metis_tac[]
+    ) >>
+  (
+    pop_assum kall_tac >>
+    simp[COND_RAND, COND_RATOR, SF CONJ_ss] >>
+    gvs[MAP_MAP_o, combinTheory.o_DEF, UNCURRY, FORALL_PROD] >>
+    simp[BIGUNION_SUBSET, MEM_MAP, PULL_EXISTS, EXISTS_PROD] >>
+    eq_tac >> rw[] >> gvs[]
+    >- metis_tac[]
+    >- metis_tac[]
+    >- gvs[allvars_IfDisj, COND_RAND, COND_RATOR]
+    >- (CASE_TAC >> gvs[] >> CASE_TAC >> gvs[allvars_IfDisj] >> rw[])
+    >- metis_tac[]
+    >- metis_tac[]
+  )
+QED
+
+(* Helper for mlmap theorems *)
+fun cjs th =
+  let fun generate_list f seed =
+          if not (can f seed) then []
+          else let val (e, seed') = f seed
+               in e :: (generate_list f seed') end
+  in generate_list (fn i => (cj i th, i + 1)) 1 end;
+
+Theorem freshen_aux_avoid_ok:
+  (∀varmap (ce1:'a cexp) avoid1 ce2 avoid2.
+    freshen_aux varmap ce1 avoid1 = (ce2,avoid2) ∧
+    avoid_ok avoid1 ce1
+   ⇒ avoid_ok avoid2 ce2) ∧
+  (∀varmap (ces1:'a cexp list) avoid1 ces2 avoid2.
+    freshen_aux_list varmap ces1 avoid1 = (ces2,avoid2) ∧
+    EVERY (avoid_ok avoid1) ces1
+   ⇒ EVERY (avoid_ok avoid2) ces2)
+Proof
+  ho_match_mp_tac freshen_aux_ind >> rw[freshen_aux_def] >> gvs[]
+  >- ( (* Var *)
+    gvs[avoid_ok_def, exp_of_def] >> CASE_TAC >> gvs[] >> res_tac
+    )
+  >- ( (* Prim *)
+    rpt (pairarg_tac >> gvs[]) >>
+    first_x_assum drule >> strip_tac >> gvs[] >>
+    Cases_on `ces1` >> gvs[freshen_aux_def] >> rpt (pairarg_tac >> gvs[]) >>
+    gvs[avoid_ok_def]
+    )
+  >- ( (* App *)
+    rpt (pairarg_tac >> gvs[]) >>
+    last_x_assum drule >> simp[] >> strip_tac >>
+    last_x_assum drule >> impl_tac
+    >- (
+      gvs[avoid_ok_def, EVERY_MEM] >>
+      drule_all $ cj 1 freshen_aux_mono >> metis_tac[SUBSET_DEF]
+      ) >>
+    gvs[avoid_ok_def] >>
+    drule_all $ cj 2 freshen_aux_mono >> strip_tac >> metis_tac[SUBSET_DEF]
+    )
+  >- ( (* Lam *)
+    rpt (pairarg_tac >> gvs[]) >> gvs[avoid_ok_def] >>
+    dxrule_all fresh_boundvars_vars >> strip_tac >>
+    last_x_assum drule >> simp[] >> impl_tac >> simp[]
+    >- (gvs[SUBSET_DEF, MEM_MAP, PULL_EXISTS] >> metis_tac[])
+    >- (drule_all $ cj 1 freshen_aux_mono >> strip_tac >> gvs[SUBSET_DEF])
+    )
+  >- ( (* Let *)
+    rpt (pairarg_tac >> gvs[]) >> gvs[avoid_ok_def, exp_of_def] >>
+    first_x_assum drule_all >> strip_tac >>
+    drule_all $ cj 1 freshen_aux_mono >> strip_tac >>
+    drule_all fresh_boundvar_vars >> strip_tac >>
+    drule_all $ cj 1 freshen_aux_mono >> strip_tac >>
+    last_x_assum drule >> simp[] >> impl_tac >> simp[]
+    >- (gvs[SUBSET_DEF] >> metis_tac[]) >>
+    strip_tac >> gvs[SUBSET_DEF]
+    )
+  >- ( (* Letrec *)
+    rpt (pairarg_tac >> gvs[]) >> gvs[avoid_ok_def] >>
+    DEP_REWRITE_TAC $ cjs MAP_ZIP >>
+    imp_res_tac freshen_mapM_LENGTH >> simp[] >>
+    imp_res_tac fresh_boundvars_LENGTH >> simp[] >>
+    rename1 `freshen_aux _ ce1 avoid3 = (ce2,avoid4)` >>
+    rename1 `freshen_mapM _ fns avoid2 = (fns',_)` >>
+    rename1 `fresh_boundvars _ _ _ = ((freshes,_),_)` >>
+    drule_all fresh_boundvars_vars >> strip_tac >>
+    DEP_REWRITE_TAC $ cjs $ SRULE [LAMBDA_PROD] every_zip_snd >>
+    qsuff_tac
+      `vars_ok avoid3 ∧ set_of avoid2 ⊆ set_of avoid3 ∧
+       EVERY (λce. allvars (exp_of ce) ⊆ set_of avoid3) fns'`
+     >- (
+      strip_tac >> last_x_assum drule >> simp[] >> impl_tac
+      >- (gvs[SUBSET_DEF, EXTENSION, MEM_MAP] >> metis_tac[]) >>
+      strip_tac >> simp[] >>
+      drule_all $ cj 1 freshen_aux_mono >> strip_tac >>
+      gvs[SUBSET_DEF, EXTENSION, EVERY_MEM] >> metis_tac[]
+      ) >>
+    `EVERY (λ(f,ce). allvars (exp_of ce) ⊆ set_of avoid2) fns` by (
+      gvs[EVERY_MEM, FORALL_PROD, SUBSET_DEF] >> metis_tac[]) >>
+    qpat_x_assum `set_of avoid2 = _` kall_tac >>
+    map_every (fn p => qpat_x_assum p mp_tac)
+      [`freshen_mapM _ _ _ = _`,`vars_ok avoid2`,`EVERY _ fns`,
+       `∀f ce vm. _`] >>
+    rpt $ pop_assum kall_tac >> strip_tac >>
+    map_every qid_spec_tac [`avoid2`,`fns'`] >>
+    Induct_on `fns` >- rw[freshen_mapM_def] >>
+    rpt gen_tac >> strip_tac >> rpt gen_tac >>
+    PairCases_on `h` >> simp[freshen_mapM_def] >> simp[AND_IMP_INTRO] >> strip_tac >>
+    qpat_x_assum `∀f ce vm. _` mp_tac >>
+    simp[DISJ_IMP_THM, FORALL_AND_THM] >> strip_tac >>
+    last_x_assum dxrule >> strip_tac >>
+    pairarg_tac >> last_x_assum drule_all >> strip_tac >>
+    rpt (pairarg_tac >> gvs[]) >>
+    first_x_assum $ drule_at $ Pat `freshen_mapM` >> impl_tac
+    >- (
+      drule_all $ cj 1 freshen_aux_mono >> strip_tac >>
+      gvs[EVERY_MEM, SUBSET_DEF, FORALL_PROD] >> metis_tac[]
+      ) >>
+    strip_tac >> simp[] >>
+    drule_all $ cj 1 freshen_aux_mono >> strip_tac >> metis_tac[SUBSET_DEF]
+    )
+  >- ( (* Case *)
+    rpt (pairarg_tac >> gvs[]) >>
+    rename1 `avoid_ok avoid5 _ ∧ _` >>
+    rename1 `freshen_mapM _ css1 avoid3 = (css2,avoid4)` >>
+    rename1 `fresh_boundvar x _ avoid2 = ((y,varmap'), _)` >>
+    rename1 `freshen_aux _ _ _ = (ce2,avoid2)` >>
+    first_x_assum $ drule_all >> strip_tac >>
+    drule fresh_boundvar_vars >> impl_tac >- fs[avoid_ok_def] >> strip_tac >>
+    drule $ cj 1 freshen_aux_mono >> impl_tac >- gvs[avoid_ok_def] >> strip_tac >>
+    `EVERY (λ(cn,pvs,ce).
+      set (MAP explode pvs) ⊆ set_of avoid3 ∧ avoid_ok avoid3 ce) css1` by (
+        gvs[EVERY_MEM, EVERY_MAP, FORALL_PROD] >>
+        gvs[SUBSET_DEF, EXTENSION, avoid_ok_def] >> metis_tac[]) >>
+    qsuff_tac
+      `set_of avoid3 ⊆ set_of avoid4 ∧ vars_ok avoid4 ∧
+       EVERY (λ(cn,pvs,ce).
+        set (MAP explode pvs) ⊆ set_of avoid4 ∧ avoid_ok avoid4 ce) css2`
+    >- (
+      strip_tac >> namedCases_on `usopt` ["","us"] >> gvs[]
+      >- (gvs[SUBSET_DEF, avoid_ok_def]) >>
+      PairCases_on `us` >> gvs[] >> rpt (pairarg_tac >> gvs[]) >>
+      last_x_assum drule >> impl_tac >- gvs[avoid_ok_def, SUBSET_DEF] >>
+      strip_tac >> simp[] >>
+      drule_all $ cj 1 freshen_aux_mono >> strip_tac >>
+      gvs[EVERY_MEM, FORALL_PROD, SUBSET_DEF, avoid_ok_def] >> metis_tac[]
+      ) >>
+    pop_assum mp_tac >>
+    map_every (fn p => qpat_x_assum p mp_tac)
+      [`freshen_mapM _ _ _ = _`,`vars_ok avoid3`,`∀cn pvs ce vm. _`] >>
+    rpt $ pop_assum kall_tac >> strip_tac >>
+    map_every qid_spec_tac [`avoid3`,`css2`] >>
+    Induct_on `css1` >> simp[freshen_mapM_def, AND_IMP_INTRO] >>
+    simp[DISJ_IMP_THM, FORALL_AND_THM] >>
+    gen_tac >> strip_tac >> rpt gen_tac >> strip_tac >>
+    last_x_assum dxrule >> strip_tac >>
+    rpt (pairarg_tac >> gvs[]) >>
+    rename1 `fresh_boundvars _ _ avoid1 = (_,avoid2)` >>
+    rename1 `freshen_aux _ _ _ = (_,avoid3)` >>
+    drule_all fresh_boundvars_vars >> strip_tac >>
+    last_x_assum drule >> impl_tac >- (gvs[avoid_ok_def, SUBSET_DEF]) >> strip_tac >>
+    drule_all $ cj 1 freshen_aux_mono >> strip_tac >>
+    last_x_assum $ drule_at $ Pat `freshen_mapM` >> reverse impl_tac >> simp[]
+    >- (strip_tac >> gvs[SUBSET_DEF, avoid_ok_def]) >>
+    gvs[EVERY_MEM, FORALL_PROD, avoid_ok_def, SUBSET_DEF, EXTENSION] >> metis_tac[]
+    )
+  >- ( (* list case *)
+    rpt (pairarg_tac >> gvs[]) >>
+    last_x_assum drule_all >> strip_tac >> drule $ cj 1 freshen_aux_mono >>
+    impl_tac >- gvs[avoid_ok_def] >> strip_tac >> gvs[] >>
+    last_x_assum drule >> impl_tac
+    >- (gvs[EVERY_MEM, avoid_ok_def] >> metis_tac[SUBSET_DEF]) >>
+    strip_tac >> simp[] >>
+    drule $ cj 2 freshen_aux_mono >> gvs[avoid_ok_def, SUBSET_DEF]
+    )
+QED
+
+Theorem freshen_aux_cns_arities:
+  (∀m (ce1:'a cexp) avoid1 ce2 avoid2.
+    freshen_aux m ce1 avoid1 = (ce2, avoid2)
+  ⇒ cns_arities ce2 = cns_arities ce1) ∧
+  (∀m (ces1:'a cexp list) avoid1 ces2 avoid2.
+    freshen_aux_list m ces1 avoid1 = (ces2, avoid2)
+  ⇒ LIST_REL (λce1 ce2. cns_arities ce2 = cns_arities ce1) ces1 ces2)
+Proof
+  ho_match_mp_tac freshen_aux_ind >>
+  rw[freshen_return_def, freshen_bind_def, freshen_aux_def, cns_arities_def] >>
+  gvs[combinTheory.o_DEF] >> rpt (pairarg_tac >> gvs[]) >> gvs[cns_arities_def] >>
+  rpt $ first_x_assum drule >> rw[]
+  >- (
+    gvs[LIST_REL_EL_EQN] >>
+    ntac 3 AP_TERM_TAC >> rw[MAP_EQ_EVERY2, LIST_REL_EL_EQN]
+    )
+  >- (
+    ntac 3 AP_TERM_TAC >> gvs[MAP_EQ_EVERY2, LIST_REL_EL_EQN]
+    )
+  >- (
+    imp_res_tac fresh_boundvars_LENGTH >> gvs[] >>
+    imp_res_tac freshen_mapM_LENGTH >> gvs[] >>
+    AP_THM_TAC >> ntac 3 AP_TERM_TAC >>
+    simp[SRULE [combinTheory.o_DEF, LAMBDA_PROD] MAP_ZIP] >>
+    qpat_x_assum `freshen_mapM _ _ _ = _` mp_tac >>
+    last_x_assum mp_tac >> rpt $ pop_assum kall_tac >> strip_tac >>
+    rename1 `freshen_mapM _ _ avoid = (fns',avoid2)` >>
+    map_every qid_spec_tac [`fns'`,`avoid`]  >>
+    Induct_on `fns` >> rw[freshen_mapM_def] >>
+    rpt (pairarg_tac >> gvs[]) >> gvs[SF DNF_ss] >>
+    first_x_assum drule >> rw[] >>
+    last_x_assum drule_all >> rw[]
+    )
+  >- (
+    rename1 `freshen_mapM _ css avoid = (css',avoid')` >>
+    `LIST_REL (λ(cn,vs,e) (cn',vs',e').
+        cn = cn' ∧ LENGTH vs = LENGTH vs' ∧ cns_arities e = cns_arities e') css css'`
+      by (
+        qpat_x_assum `freshen_mapM _ _ _ = _` mp_tac >>
+        last_x_assum mp_tac >> rpt $ pop_assum kall_tac >> strip_tac >>
+        map_every qid_spec_tac [`css'`,`avoid`] >>
+        Induct_on `css` >> rw[freshen_mapM_def] >>
+        rpt (pairarg_tac >> gvs[]) >> gvs[SF DNF_ss] >>
+        imp_res_tac fresh_boundvars_LENGTH >> simp[] >>
+        first_x_assum drule >> rw[] >> last_x_assum drule_all >> simp[]) >>
+    `MAP (λ(cn,vs,e). (cn,LENGTH vs)) css' =
+     MAP (λ(cn,vs,e). (cn,LENGTH vs)) css` by (
+      rw[MAP_EQ_EVERY2] >> gvs[LIST_REL_EL_EQN] >> rw[] >>
+      first_x_assum drule >> rpt (pairarg_tac >> gvs[])) >>
+    `MAP (λ(cn,vs,e). cns_arities e) css' =
+     MAP (λ(cn,vs,e). cns_arities e) css` by (
+      rw[MAP_EQ_EVERY2] >> gvs[LIST_REL_EL_EQN] >> rw[] >>
+      first_x_assum drule >> rpt (pairarg_tac >> gvs[])) >>
+     simp[] >> AP_THM_TAC >> AP_TERM_TAC >>
+     namedCases_on `usopt` ["","us"] >> gvs[] >>
+     PairCases_on `us` >> gvs[] >> pairarg_tac >> gvs[] >>
+     last_x_assum drule >> simp[]
+    )
+QED
+
+Theorem freshen_aux_cexp_wf:
+  (∀m (ce1:'a cexp) avoid1 ce2 avoid2.
+    freshen_aux m ce1 avoid1 = (ce2, avoid2) ∧ vars_ok avoid1 ∧ cexp_wf ce1
+    ⇒ cexp_wf ce2) ∧
+  (∀m (ces1:'a cexp list) avoid1 ces2 avoid2.
+    freshen_aux_list m ces1 avoid1 = (ces2, avoid2) ∧ vars_ok avoid1 ∧
+    EVERY cexp_wf ces1
+  ⇒ EVERY cexp_wf ces2)
+Proof
+  ho_match_mp_tac freshen_aux_ind >>
+  rw[freshen_return_def, freshen_bind_def, freshen_aux_def, cexp_wf_def] >>
+  gvs[combinTheory.o_DEF] >> rpt (pairarg_tac >> gvs[]) >>
+  gvs[cexp_wf_def, SF ETA_ss] >>
+  rpt $ (first_x_assum drule_all >> strip_tac) >> gvs[]
+  >- (imp_res_tac freshen_aux_list_LENGTH >> gvs[])
+  >- (
+    last_x_assum $ irule_at Any >> goal_assum drule >>
+    imp_res_tac freshen_aux_list_LENGTH >> Cases_on `ces'` >> gvs[] >>
+    dxrule_all $ cj 1 freshen_aux_mono >> rw[]
+    )
+  >- (
+    last_x_assum $ irule_at Any >> goal_assum drule >>
+    imp_res_tac fresh_boundvars_LENGTH >> Cases_on `vs'` >> gvs[] >>
+    drule_all fresh_boundvars_vars >> strip_tac
+    )
+  >- (
+    last_x_assum irule >> goal_assum $ drule_at Any >>
+    drule_all $ cj 1 freshen_aux_mono >> rw[] >>
+    drule_all fresh_boundvar_vars >> simp[]
+    )
+  >- (
+    rename1 `freshen_aux _ ce1 avoid3 = (ce2,avoid4)` >>
+    rename1 `freshen_mapM _ _ avoid2 = (fns',_)` >>
+    rename1 `fresh_boundvars _ _ _ = ((freshes,_),_)` >>
+    imp_res_tac fresh_boundvars_LENGTH >>
+    imp_res_tac freshen_mapM_LENGTH >>
+    last_x_assum $ irule_at Any >> goal_assum drule >>
+    dxrule_all fresh_boundvars_vars >> strip_tac >> simp[MAP_ZIP] >>
+    once_rewrite_tac[CONJ_ASSOC] >> reverse conj_tac
+    >- (
+      Cases_on `fns` >> gvs[] >>
+      Cases_on `freshes` >> gvs[] >> Cases_on `fns'` >> gvs[]
+      ) >>
+    qpat_x_assum `freshen_mapM _ _ _ = _` mp_tac >>
+    qpat_x_assum `EVERY cexp_wf _` mp_tac >>
+    qpat_x_assum `vars_ok avoid2` mp_tac >>
+    last_x_assum mp_tac >> rpt $ pop_assum kall_tac >> strip_tac >>
+    map_every qid_spec_tac [`avoid2`,`fns'`] >>
+    Induct_on `fns` >> simp[freshen_mapM_def, AND_IMP_INTRO] >>
+    gen_tac >> strip_tac >> rpt gen_tac >> strip_tac >>
+    gvs[DISJ_IMP_THM, FORALL_AND_THM] >>
+    last_x_assum drule >> strip_tac >>
+    rpt (pairarg_tac >> gvs[]) >> PairCases_on `h` >> gvs[] >>
+    first_x_assum drule_all >> strip_tac >> simp[] >>
+    first_x_assum irule >> goal_assum $ drule_at $ Pat `freshen_mapM` >>
+    drule_all $ cj 1 freshen_aux_mono >> rw[]
+    )
+  >- (
+    rename1 `freshen_mapM _ css avoid = (css',avoid')` >>
+    `LIST_REL (λ(cn,vs,e) (cn',vs',e').
+        cn = cn' ∧ LENGTH vs = LENGTH vs' ∧ cexp_wf e' ∧
+        ALL_DISTINCT vs' ∧ ¬MEM v' vs') css css' ∧ vars_ok avoid'`
+      by (
+        qpat_x_assum `freshen_mapM _ _ _ = _` mp_tac >>
+        qpat_x_assum `EVERY cexp_wf _` mp_tac >>
+        `vars_ok avoid ∧ explode v' ∈ set_of avoid` by (
+          drule_all $ cj 1 freshen_aux_mono >> strip_tac >>
+          drule_all $ fresh_boundvar_vars >> rw[]) >>
+        ntac 2 $ pop_assum mp_tac >>
+        last_x_assum mp_tac >> rpt $ pop_assum kall_tac >> strip_tac >>
+        map_every qid_spec_tac [`css'`,`avoid`] >>
+        Induct_on `css` >> simp[freshen_mapM_def, AND_IMP_INTRO] >>
+        gen_tac >> strip_tac >> rpt gen_tac >> strip_tac >>
+        gvs[DISJ_IMP_THM, FORALL_AND_THM] >>
+        last_x_assum drule >> strip_tac >>
+        rpt (pairarg_tac >> gvs[]) >>
+        last_x_assum $ dxrule_at $ Pat `freshen_mapM` >> strip_tac >>
+        gvs[UNCURRY] >> simp[FST_THM] >> pairarg_tac >> gvs[] >>
+        drule_all fresh_boundvars_vars >> strip_tac >>
+        last_x_assum drule_all >> strip_tac >> simp[] >>
+        imp_res_tac fresh_boundvars_LENGTH >> simp[] >>
+        simp[GSYM CONJ_ASSOC] >> conj_tac
+        >- (gvs[DISJOINT_ALT, MEM_MAP, PULL_EXISTS] >> metis_tac[]) >>
+        first_x_assum irule >> drule_all $ cj 1 freshen_aux_mono >> gvs[SUBSET_DEF]) >>
+    `MAP FST css' = MAP FST css` by (
+      rw[MAP_EQ_EVERY2] >> gvs[LIST_REL_EL_EQN] >> rw[] >>
+      first_x_assum drule >> rpt (pairarg_tac >> gvs[])) >>
+    `css' ≠ []` by (Cases_on `css` >> gvs[]) >> simp[] >> conj_tac
+    >- (
+      gvs[EVERY_MAP, EVERY_EL, LIST_REL_EL_EQN] >>
+      rw[] >> first_x_assum drule >> rpt (pairarg_tac >> gvs[])
+      ) >>
+    qsuff_tac `EVERY ALL_DISTINCT (MAP (FST o SND) css') ∧
+              ¬MEM v' (FLAT (MAP (FST o SND) css'))`
+    >- (
+      simp[] >> strip_tac >> namedCases_on `usopt` ["","us"] >> gvs[] >>
+      PairCases_on `us` >> gvs[UNCURRY] >> simp[FST_THM] >> pairarg_tac >> gvs[] >>
+      first_x_assum drule >> simp[]
+      ) >>
+    simp[EVERY_MAP, EVERY_EL, MEM_FLAT, DISJ_EQ_IMP] >>
+    simp[Once MEM_EL, PULL_EXISTS, EL_MAP] >>
+    rw[] >> gvs[LIST_REL_EL_EQN] >>
+    first_x_assum drule >> rpt (pairarg_tac >> gvs[])
+    )
+  >- gvs[combinTheory.o_DEF]
+  >- (
+    first_x_assum irule >> goal_assum $ drule_at Any >>
+    drule_all $ cj 1 freshen_aux_mono >> rw[]
+    )
+QED
+
+Theorem freshen_aux_NestedCase_free:
+  (∀m (ce1:'a cexp) avoid1 ce2 avoid2.
+    freshen_aux m ce1 avoid1 = (ce2, avoid2) ∧ NestedCase_free ce1
+  ⇒ NestedCase_free ce2) ∧
+  (∀m (ces1:'a cexp list) avoid1 ces2 avoid2.
+    freshen_aux_list m ces1 avoid1 = (ces2, avoid2) ∧
+    EVERY NestedCase_free ces1
+  ⇒ EVERY NestedCase_free ces2)
+Proof
+  ho_match_mp_tac freshen_aux_ind >>
+  rw[freshen_return_def, freshen_bind_def, freshen_aux_def, NestedCase_free_def] >>
+  gvs[combinTheory.o_DEF] >> rpt (pairarg_tac >> gvs[]) >> gvs[NestedCase_free_def] >>
+  rpt $ first_x_assum drule >> rw[] >> gvs[SF ETA_ss]
+  >- (
+    imp_res_tac fresh_boundvars_LENGTH >>
+    imp_res_tac freshen_mapM_LENGTH >> simp[MAP_ZIP] >>
+    qpat_x_assum `freshen_mapM _ _ _ = _` mp_tac >>
+    qpat_x_assum `EVERY _ _` mp_tac >>
+    last_x_assum mp_tac >> rpt $ pop_assum kall_tac >> strip_tac >>
+    map_every qid_spec_tac [`x`,`fces'`] >>
+    Induct_on `fns` >> rw[freshen_mapM_def] >>
+    rpt (pairarg_tac >> gvs[]) >> gvs[SF DNF_ss] >> PairCases_on `h` >> gvs[] >>
+    first_x_assum drule >> rw[] >> last_x_assum drule_all >> simp[]
+    )
+  >- (
+    qpat_x_assum `freshen_mapM _ _ _ = _` mp_tac >>
+    qpat_x_assum `EVERY _ _` mp_tac >>
+    last_x_assum mp_tac >> rpt $ pop_assum kall_tac >> strip_tac >>
+    map_every qid_spec_tac [`x'`,`css'`] >>
+    Induct_on `css` >> rw[freshen_mapM_def] >>
+    rpt (pairarg_tac >> gvs[]) >> gvs[SF DNF_ss] >>
+    last_x_assum drule_all >> rw[] >>
+    gvs[UNCURRY] >> simp[FST_THM] >> pairarg_tac >> gvs[] >>
+    first_x_assum drule >> simp[]
+    )
+  >- (
+    namedCases_on `usopt` ["","us"] >> gvs[] >>
+    PairCases_on `us` >> gvs[] >>
+    gvs[UNCURRY] >> simp[FST_THM] >> pairarg_tac >> gvs[] >>
+    first_x_assum drule >> rw[]
+    )
+QED
+
+
+(********** relating freshen_aux and freshen_global **********)
+
+Definition varmap_rel_def:
+  varmap_rel varmap fmap ⇔
+    map_ok varmap ∧ cmp_of varmap = var_cmp ∧
+    (∀k v. lookup varmap k = SOME v ⇔
+      FLOOKUP fmap (explode k) = SOME (explode v))
+End
+
+Theorem fresh_boundvar_rel:
+  varmap_rel varmap m ∧
+  vars_ok avoid ∧
+  fresh_boundvar x varmap avoid = ((y,varmap'), avoid')
+  ⇒ varmap_rel varmap' (m |+ (explode x,explode y)) ∧
+    explode y ∉ set_of avoid ∧
+    set_of avoid' = explode y INSERT set_of avoid ∧
+    vars_ok avoid'
+Proof
+  strip_tac >> gvs[fresh_boundvar_def] >> rpt (pairarg_tac >> gvs[]) >>
+  drule_all invent_var_thm >> strip_tac >> gvs[varmap_rel_def] >>
+  DEP_REWRITE_TAC $ cjs mlmapTheory.insert_thm >> simp[] >> rw[] >>
+  DEP_REWRITE_TAC[mlmapTheory.lookup_insert] >> simp[FLOOKUP_SIMP] >>
+  IF_CASES_TAC >> gvs[]
+QED
+
+Theorem fresh_boundvars_rel:
+  ∀xs varmap avoid ys varmap' avoid' m.
+  varmap_rel varmap m ∧
+  vars_ok avoid ∧
+  fresh_boundvars xs varmap avoid = ((ys,varmap'), avoid')
+  ⇒ LENGTH xs = LENGTH ys ∧
+    varmap_rel varmap' (m |++ ZIP (MAP explode xs, MAP explode ys)) ∧
+    set_of avoid' = set (MAP explode ys) ∪ set_of avoid ∧
+    ALL_DISTINCT ys ∧
+    DISJOINT (set (MAP explode ys)) (set_of avoid) ∧
+    vars_ok avoid'
+Proof
+  Induct >> rpt gen_tac >> strip_tac >> gvs[fresh_boundvars_def]
+  >- simp[FUPDATE_LIST_THM] >>
+  rpt (pairarg_tac >> gvs[]) >> simp[FUPDATE_LIST_THM] >>
+  dxrule_all fresh_boundvar_rel >> strip_tac >>
+  last_x_assum drule_all >> simp[] >> strip_tac >>
+  gvs[MEM_MAP] >>
+  rw[EXTENSION] >> eq_tac >> rw[] >> metis_tac[]
+QED
+
+Theorem freshen_aux_freshen_global:
+  (∀varmap (ce1:'a cexp) avoid1 ce2 avoid2 m.
+    freshen_aux varmap ce1 avoid1 = (ce2,avoid2) ∧
+    varmap_rel varmap m ∧ avoid_ok avoid1 ce1 ∧
+    NestedCase_free ce1 ∧ letrecs_distinct (exp_of ce1) ∧ cexp_wf ce1
+   ⇒ freshen_global (set_of avoid1) m (exp_of ce1) (exp_of ce2)) ∧
+
+  (∀varmap (ces1:'a cexp list) avoid1 ces2 avoid4 m.
+    freshen_aux_list varmap ces1 avoid1 = (ces2,avoid4) ⇒
+    ∀l1 ce1 r1 l2 avoid2 ce2 avoid3.
+      ces1 = l1 ++ [ce1] ++ r1 ∧
+      freshen_aux_list varmap l1 avoid1 = (l2,avoid2) ∧
+      freshen_aux varmap ce1 avoid2 = (ce2,avoid3) ∧
+      varmap_rel varmap m ∧ EVERY (avoid_ok avoid1) (l1 ++ [ce1]) ∧
+      EVERY NestedCase_free (l1 ++ [ce1]) ∧
+      EVERY letrecs_distinct (MAP exp_of l1 ++ [exp_of ce1]) ∧
+      EVERY cexp_wf (l1 ++ [ce1])
+    ⇒ ∃r2. ces2 = l2 ++ [ce2] ++ r2 ∧
+        freshen_global (set_of avoid2) m (exp_of ce1) (exp_of ce2))
+Proof
+  ho_match_mp_tac freshen_aux_ind >>
+  rw[freshen_aux_def] >> gvs[exp_of_def]
+  >- ( (* Var *)
+    simp[Once freshen_global_cases] >>
+    CASE_TAC >> gvs[varmap_rel_def] >>
+    Cases_on `FLOOKUP m (explode v)` >> gvs[] >>
+    `∃x'. x = explode x'` by (qexists `implode x` >> simp[]) >> gvs[] >>
+    first_x_assum $ drule o iffRL >> simp[]
+    )
+  >- ( (* Prim *)
+    simp[Once freshen_global_cases] >>
+    pairarg_tac >> gvs[exp_of_def, cexp_wf_def, letrecs_distinct_def, SF ETA_ss] >>
+    imp_res_tac freshen_aux_list_LENGTH >> rw[] >>
+    gvs[MAP_EQ_APPEND, PULL_EXISTS] >> rename1 `l ++ [ce] ++ r` >>
+    last_x_assum drule >>
+    disch_then $ qspecl_then [`m`,`l`] mp_tac >> simp[] >>
+    gvs[freshen_aux_list_append, freshen_aux_def] >>
+    rpt (pairarg_tac >> gvs[]) >> strip_tac >>
+    irule_at Any EQ_REFL >> imp_res_tac freshen_aux_list_LENGTH >> simp[] >>
+    irule freshen_global_mono >> goal_assum $ drule_at Any >>
+    rev_drule_all $ cj 2 freshen_aux_avoid_ok >> strip_tac >> rw[]
+    >- (rev_drule $ cj 2 freshen_aux_mono >> gvs[]) >>
+    simp[BIGUNION_SUBSET, MEM_MAP, PULL_EXISTS, FORALL_PROD] >>
+    gvs[EVERY_MEM, avoid_ok_def, allvars_thm]
+    )
+  >- ( (* App *)
+    rpt (pairarg_tac >> gvs[]) >>
+    gvs[exp_of_def, cexp_wf_def, letrecs_distinct_Apps, SF ETA_ss] >>
+    rename1 `freshen_aux_list _ ces1 _ = (ces2, avoid3)` >>
+    rename1 `freshen_aux _ ce1 _ = (ce2, avoid2)` >>
+    last_x_assum drule_all >> strip_tac >>
+    last_x_assum drule >> strip_tac >>
+    `EVERY (avoid_ok avoid2) ces1` by (
+      drule $ cj 1 freshen_aux_mono >>
+      gvs[avoid_ok_def, EVERY_MEM, SUBSET_DEF] >> metis_tac[]) >>
+    `set_of avoid1 ⊆ set_of avoid2 ∧ avoid_ok avoid2 ce2` by (
+      drule $ cj 1 freshen_aux_mono >> gvs[avoid_ok_def] >>
+      drule $ cj 1 freshen_aux_avoid_ok >> gvs[avoid_ok_def]) >>
+    map_every (fn p => qpat_x_assum p kall_tac)
+      [`freshen_aux _ _ _ = _`, `EVERY (avoid_ok avoid1) _`, `_ ≠ []`,
+       `NestedCase_free ce1`,`letrecs_distinct (exp_of ce1)`,`cexp_wf ce1`] >>
+    rpt $ pop_assum mp_tac >>
+    map_every qid_spec_tac [`ces2`,`avoid3`] >>
+    Induct_on `ces1` using SNOC_INDUCT >> rw[] >> gvs[SNOC_APPEND]
+    >- gvs[freshen_aux_def, Apps_def] >>
+    gvs[Apps_append, freshen_aux_list_append, freshen_aux_def] >>
+    rpt (pairarg_tac >> gvs[]) >> gvs[Apps_append, Apps_def] >>
+    simp[Once freshen_global_cases] >> disj1_tac >> reverse $ rw[]
+    >- (
+      first_x_assum $ qspecl_then [`m`,`ces1`] mp_tac >> simp[] >>
+      strip_tac >> irule freshen_global_mono >> goal_assum $ drule_at Any >>
+      rev_drule $ cj 2 freshen_aux_mono >> strip_tac >>
+      rev_drule_all $ cj 2 freshen_aux_avoid_ok >> strip_tac >>
+      gvs[avoid_ok_def, boundvars_Apps, allvars_thm,
+          SUBSET_DEF, EVERY_MEM, MEM_MAP, PULL_EXISTS] >>
+      rw[] >> gvs[] >> metis_tac[]
+      )
+    >- (
+      last_x_assum irule >> rw[] >> gvs[] >>
+      last_x_assum $ qspecl_then [`m'`,`l1`] mp_tac >> rw[] >>
+      gvs[freshen_aux_list_append, freshen_aux_def] >> rpt (pairarg_tac >> gvs[])
+      )
+    )
+  >- ( (* Lams *)
+    rpt (pairarg_tac >> gvs[]) >>
+    gvs[exp_of_def, letrecs_distinct_Lams, cexp_wf_def] >>
+    last_x_assum drule >> strip_tac >>
+    irule freshen_global_Lams >>
+    drule fresh_boundvars_rel >> rpt $ disch_then $ drule_at Any >>
+    gvs[avoid_ok_def] >> strip_tac >>
+    irule_at Any freshen_global_mono >> first_x_assum $ irule_at Any >> simp[] >>
+    gvs[SUBSET_DEF]
+    )
+  >- ( (* Let *)
+    rpt (pairarg_tac >> gvs[]) >> gvs[exp_of_def, letrecs_distinct_def, cexp_wf_def] >>
+    rename1 `freshen_aux varmap1 ce2 avoid3 = (ce2',avoid4)` >>
+    rename1 `freshen_aux varmap ce1 _ = (ce1',avoid2)` >>
+    first_x_assum drule_all >> strip_tac >>
+    simp[Once freshen_global_cases] >> disj2_tac >>
+    drule_all $ cj 1 freshen_aux_avoid_ok >> strip_tac >>
+    rev_drule $ cj 1 freshen_aux_mono >> strip_tac >>
+    drule fresh_boundvar_rel >> rpt $ disch_then $ drule_at Any >>
+    impl_tac >- gvs[avoid_ok_def] >> strip_tac >> rw[]
+    >- (gvs[avoid_ok_def, SUBSET_DEF] >> CCONTR_TAC >> gvs[allvars_thm])
+    >- (gvs[avoid_ok_def, SUBSET_DEF] >> CCONTR_TAC >> gvs[allvars_thm]) >>
+    irule freshen_global_mono >> first_x_assum $ irule_at Any >>
+    rpt $ goal_assum $ drule_at Any >>
+    gvs[avoid_ok_def, SUBSET_DEF] >> gvs[allvars_thm]
+    )
+  >- ( (* Letrec *)
+    rpt (pairarg_tac >> gvs[]) >> gvs[exp_of_def, letrecs_distinct_def, cexp_wf_def] >>
+    rename1 `freshen_aux _ ce1 avoid3 = (ce2,avoid4)` >>
+    rename1 `fresh_boundvars _ _ _ = ((freshes,_),avoid2)` >>
+    rename1 `freshen_mapM _ _ _ = (fns',_)` >>
+    simp[Once freshen_global_cases] >>
+    drule fresh_boundvars_rel >> rpt $ disch_then $ drule_at Any >>
+    impl_tac >- gvs[avoid_ok_def] >> strip_tac >> gvs[] >>
+    qexists `FEMPTY |++ ZIP (MAP (explode o FST) fns, MAP explode freshes)` >>
+    rw[]
+    >- simp[FDOM_FUPDATE_LIST, MAP_MAP_o, combinTheory.o_DEF, LAMBDA_PROD, MAP_ZIP]
+    >- (
+      simp[Once DISJOINT_SYM] >> irule DISJOINT_SUBSET >>
+      irule_at Any FRANGE_FUPDATE_LIST_SUBSET >> simp[MAP_ZIP]
+      )
+    >- (
+      gvs[FLOOKUP_FUPDATE_LIST, AllCaseEqs()] >>
+      gvs[MAP_MAP_o, combinTheory.o_DEF, LAMBDA_PROD] >>
+      rpt $ dxrule_then assume_tac ALOOKUP_MEM >> gvs[MEM_ZIP, EL_MAP] >>
+      gvs[EL_ALL_DISTINCT_EL_EQ, EL_MAP]
+      )
+    >- (imp_res_tac freshen_mapM_LENGTH >> gvs[])
+    >- (
+      last_x_assum kall_tac >> qpat_x_assum `freshen_aux _ _ _ = _` kall_tac >>
+      gvs[MAP_EQ_APPEND, PULL_EXISTS] >> pairarg_tac >> gvs[] >>
+      rename1 `l ++ [f1,fce1] ++ r` >>
+      gvs[DISJ_IMP_THM, FORALL_AND_THM] >>
+      qpat_x_assum `∀f ce vm. MEM _ r ⇒ _` kall_tac >>
+      gvs[freshen_mapM_append, freshen_mapM_def,
+          fresh_boundvars_append, fresh_boundvars_def] >>
+      rpt (pairarg_tac >> gvs[]) >>
+      imp_res_tac fresh_boundvars_LENGTH >> imp_res_tac freshen_mapM_LENGTH >>
+      gvs[] >>
+      rename1 `ZIP (fresh_l ++ [y] ++ fresh_r, fns'_l ++ [fn'] ++ fns'_r)` >>
+      simp[GSYM ZIP_APPEND] >> irule_at Any EQ_REFL >> rw[]
+      >- (
+        simp[FLOOKUP_FUPDATE_LIST, REVERSE_APPEND, ALOOKUP_APPEND, AllCaseEqs()] >>
+        disj1_tac >> qpat_x_assum `ALL_DISTINCT (_ ++ [explode _] ++ _)` mp_tac >>
+        simp[MAP_MAP_o, combinTheory.o_DEF, LAMBDA_PROD, ALL_DISTINCT_APPEND] >>
+        simp[ALOOKUP_NONE, MAP_REVERSE, MAP_ZIP] >> simp[MEM_MAP, FORALL_PROD]
+        ) >>
+      first_x_assum drule >> disch_then drule >> rename1 `avoid_ok avoid2'` >>
+      `EVERY (avoid_ok avoid2) (MAP SND l)` by (
+        gvs[EVERY_MEM, avoid_ok_def, MEM_MAP, PULL_EXISTS, FORALL_PROD, SUBSET_DEF] >>
+        metis_tac[]) >>
+      `vars_ok avoid2' ∧ set_of avoid2 ⊆ set_of avoid2' ∧
+       EVERY (avoid_ok avoid2') fns'_l` by (
+        pop_assum mp_tac >>
+        qpat_x_assum `freshen_mapM _ _ avoid2 = _` mp_tac >>
+        qpat_x_assum `vars_ok avoid2` mp_tac >> rpt $ pop_assum kall_tac >>
+        map_every qid_spec_tac [`avoid2`,`fns'_l`] >>
+        Induct_on `l` >> simp[freshen_mapM_def, AND_IMP_INTRO] >>
+        rpt gen_tac >> strip_tac >> rpt (pairarg_tac >> gvs[]) >>
+        drule_all $ cj 1 freshen_aux_mono >> strip_tac >>
+        drule_all $ cj 1 freshen_aux_avoid_ok >> strip_tac >>
+        last_x_assum drule >> rpt $ disch_then drule >>
+        impl_tac >> rw[] >>
+        gvs[avoid_ok_def, EVERY_MEM, SUBSET_DEF, MEM_MAP, PULL_EXISTS] >>
+        metis_tac[]
+        ) >>
+      impl_tac >- (rw[] >> gvs[avoid_ok_def] >> gvs[SUBSET_DEF]) >>
+      simp[MAP_MAP_o, combinTheory.o_DEF, LAMBDA_PROD, FORALL_PROD, GSYM ZIP_APPEND] >>
+      qmatch_goalsub_abbrev_tac `FRANGE (FEMPTY |++ new)` >> strip_tac >>
+      simp[SRULE [combinTheory.o_DEF, LAMBDA_PROD] MAP_ZIP] >>
+      qpat_x_assum `varmap_rel _ _` mp_tac >>
+      simp[MAP_MAP_o, combinTheory.o_DEF, LAMBDA_PROD, GSYM ZIP_APPEND] >> strip_tac >>
+      simp[GSYM fupdate_list_funion] >>
+      irule freshen_global_mono >> goal_assum $ drule_at Any >> rw[]
+      >- gvs[SUBSET_DEF]
+      >- (
+        qabbrev_tac `fresh_set =
+          set (MAP explode fresh_l) ∪ {explode y} ∪ set (MAP explode fresh_r)` >>
+        qsuff_tac `FRANGE (FEMPTY |++ new) = fresh_set` >- (strip_tac >> gvs[]) >>
+        irule SUBSET_ANTISYM >> rw[]
+        >- (
+          irule SUBSET_TRANS >> irule_at Any FRANGE_FUPDATE_LIST_SUBSET >> simp[] >>
+          unabbrev_all_tac >> gvs[MAP_ZIP, SUBSET_DEF]
+          )
+        >- (
+          irule SUBSET_TRANS >> irule_at Any FRANGE_FUPDATE_LIST_ALL_DISTINCT >>
+          unabbrev_all_tac >> simp[SUBSET_DEF] >>
+          gvs[MAP_ZIP, MAP_MAP_o, combinTheory.o_DEF, LAMBDA_PROD]
+          )
+        )
+      >- (
+        simp[BIGUNION_SUBSET, MEM_MAP, PULL_EXISTS] >>
+        gvs[EVERY_MEM, avoid_ok_def, allvars_thm]
+        )
+      )
+    >- (
+      simp[MAP_MAP_o, combinTheory.o_DEF, LAMBDA_PROD, GSYM fupdate_list_funion] >>
+      qmatch_goalsub_abbrev_tac `FRANGE (FEMPTY |++ new)` >>
+      drule freshen_mapM_LENGTH >> strip_tac >> gvs[] >>
+      simp[SRULE [combinTheory.o_DEF, LAMBDA_PROD] MAP_ZIP] >>
+      last_x_assum drule >> disch_then drule >>
+      `EVERY (avoid_ok avoid2) (MAP SND fns)` by (
+        gvs[EVERY_MEM, avoid_ok_def, MEM_MAP, PULL_EXISTS, FORALL_PROD, SUBSET_DEF] >>
+        metis_tac[]) >>
+      `vars_ok avoid3 ∧ set_of avoid2 ⊆ set_of avoid3 ∧
+       EVERY (avoid_ok avoid3) fns'` by (
+        pop_assum mp_tac >>
+        qpat_x_assum `freshen_mapM _ _ avoid2 = _` mp_tac >>
+        qpat_x_assum `vars_ok avoid2` mp_tac >> rpt $ pop_assum kall_tac >>
+        map_every qid_spec_tac [`avoid2`,`fns'`] >>
+        Induct_on `fns` >> simp[freshen_mapM_def, AND_IMP_INTRO] >>
+        rpt gen_tac >> strip_tac >> rpt (pairarg_tac >> gvs[]) >>
+        drule_all $ cj 1 freshen_aux_mono >> strip_tac >>
+        drule_all $ cj 1 freshen_aux_avoid_ok >> strip_tac >>
+        last_x_assum drule >> rpt $ disch_then drule >>
+        impl_tac >> rw[] >>
+        gvs[avoid_ok_def, EVERY_MEM, SUBSET_DEF, MEM_MAP, PULL_EXISTS, FORALL_PROD] >>
+        metis_tac[]
+        ) >>
+      impl_tac >- (rw[] >> gvs[avoid_ok_def] >> gvs[SUBSET_DEF]) >>
+      simp[MAP_MAP_o, combinTheory.o_DEF, LAMBDA_PROD] >> strip_tac >>
+      irule freshen_global_mono >> goal_assum $ drule_at Any >> rw[]
+      >- gvs[SUBSET_DEF]
+      >- (
+        qsuff_tac `FRANGE (FEMPTY |++ new) = set (MAP explode freshes)`
+        >- (strip_tac >> gvs[]) >>
+        irule SUBSET_ANTISYM >> rw[]
+        >- (
+          irule SUBSET_TRANS >> irule_at Any FRANGE_FUPDATE_LIST_SUBSET >> simp[] >>
+          unabbrev_all_tac >> gvs[MAP_ZIP]
+          )
+        >- (
+          irule SUBSET_TRANS >> irule_at Any FRANGE_FUPDATE_LIST_ALL_DISTINCT >>
+          unabbrev_all_tac >> simp[SUBSET_DEF] >>
+          gvs[MAP_ZIP, MAP_MAP_o, combinTheory.o_DEF, LAMBDA_PROD]
+          )
+        )
+      >- (
+        simp[BIGUNION_SUBSET, MEM_MAP, PULL_EXISTS] >>
+        gvs[EVERY_MEM, avoid_ok_def, allvars_thm]
+        )
+      )
+    )
+  >- ( (* Case *)
+    `¬MEM v (FLAT (MAP (FST o SND) css)) ∧ cexp_wf ce1 ∧
+     EVERY (λ(cn,pvs,ce). cexp_wf ce) css ∧ css ≠ [] ∧
+     (∀cnars us. usopt = SOME (cnars,us) ⇒ cexp_wf us)` by (
+      gvs[cexp_wf_def, combinTheory.o_DEF, LAMBDA_PROD, EVERY_MAP] >> rw[] >> gvs[]) >>
+    qpat_x_assum `cexp_wf (Case _ _ _ _ _)` kall_tac >> simp[] >>
+    rpt (pairarg_tac >> gvs[]) >>
+    gvs[exp_of_def, letrecs_distinct_rows_of, letrecs_distinct_def, cexp_wf_def] >>
+    rename1 `freshen_mapM _ css1 avoid3 = (css2,avoid4)` >>
+    rename1 `(usopt2,avoid5)` >>
+    rename1 `fresh_boundvar x _ avoid2 = ((y,_),_)` >>
+    rename1 `freshen_aux _ _ _ = (ce2,_)` >>
+    `¬ MEM y (FLAT (MAP (FST o SND) css2))` by (
+      `explode y ∈ set_of avoid3 ∧ vars_ok avoid3` by (
+        drule $ cj 1 freshen_aux_mono >> impl_tac >- gvs[avoid_ok_def] >> strip_tac >>
+        drule fresh_boundvar_vars >> simp[]) >>
+      qpat_x_assum `freshen_mapM _ _ _ = _` mp_tac >>
+      ntac 2 $ pop_assum mp_tac >> rpt $ pop_assum kall_tac >>
+      map_every qid_spec_tac [`avoid3`,`css2`] >>
+      Induct_on `css1` >> rw[freshen_mapM_def] >> rpt (pairarg_tac >> gvs[]) >>
+      drule_all fresh_boundvars_vars >> strip_tac >>
+      gvs[DISJOINT_ALT, MEM_MAP, PULL_EXISTS] >> rw[] >- metis_tac[] >>
+      first_x_assum irule >> goal_assum $ drule_at $ Pat `freshen_mapM` >>
+      drule_all $ cj 1 freshen_aux_mono >> gvs[SUBSET_DEF]) >>
+    simp[Once freshen_global_cases] >> disj2_tac >>
+    first_x_assum drule_all >> strip_tac >>
+    drule_all $ cj 1 freshen_aux_avoid_ok >> strip_tac >>
+    drule $ cj 1 freshen_aux_mono >>
+    impl_tac >- gvs[avoid_ok_def] >> strip_tac >>
+    drule_all fresh_boundvar_rel >> strip_tac >> rw[]
+    >- (CCONTR_TAC >> gvs[SUBSET_DEF])
+    >- (CCONTR_TAC >> gvs[SUBSET_DEF, avoid_ok_def, allvars_thm]) >>
+    irule freshen_global_rows_of >> simp[FLOOKUP_SIMP] >>
+    imp_res_tac freshen_mapM_LENGTH >> simp[] >> reverse conj_tac >> rw[]
+    >- (
+      namedCases_on `usopt` ["","us"] >> gvs[] >- simp[Once freshen_global_cases] >>
+      PairCases_on `us` >> gvs[] >> pairarg_tac >> gvs[] >>
+      irule freshen_global_IfDisj >> simp[FLOOKUP_SIMP] >>
+      simp[MAP_MAP_o, combinTheory.o_DEF, LAMBDA_PROD] >>
+      irule freshen_global_mono >> first_x_assum $ irule_at Any >>
+      goal_assum drule >> simp[] >>
+      qsuff_tac
+        `vars_ok avoid4 ∧ set_of avoid3 ⊆ set_of avoid4 ∧
+         EVERY (λ(cn,pvs,ce).
+            set (MAP explode pvs) ∪ boundvars (exp_of ce) ⊆ set_of avoid4) css2`
+      >- (
+        strip_tac >> gvs[avoid_ok_def, SUBSET_DEF] >>
+        conj_tac >- gvs[allvars_thm] >>
+        gvs[EVERY_MEM, MEM_MAP, PULL_EXISTS, FORALL_PROD] >> metis_tac[]
+        ) >>
+      `EVERY (λ(cn,pvs,ce).
+        set (MAP explode pvs) ⊆ set_of avoid3 ∧ avoid_ok avoid3 ce) css1` by (
+          gvs[EVERY_MEM, FORALL_PROD, SUBSET_DEF, avoid_ok_def] >>
+          metis_tac[]) >>
+      pop_assum mp_tac >>
+      map_every (fn p => qpat_x_assum p mp_tac)
+        [`freshen_mapM _ _ _ = _`,`vars_ok avoid3`] >>
+      rpt $ pop_assum kall_tac >>
+      map_every qid_spec_tac [`avoid3`,`css2`] >>
+      Induct_on `css1` >> simp[freshen_mapM_def, AND_IMP_INTRO] >>
+      rpt gen_tac >> strip_tac >> rpt (pairarg_tac >> gvs[]) >>
+      drule_all fresh_boundvars_vars >> strip_tac >>
+      drule_all $ cj 1 freshen_aux_mono >> strip_tac >> gvs[] >>
+      last_x_assum $ drule_at $ Pat `freshen_mapM` >> simp[] >> impl_tac
+      >- (gvs[EVERY_MEM, FORALL_PROD, SUBSET_DEF, avoid_ok_def] >> metis_tac[]) >>
+      drule $ cj 1 freshen_aux_avoid_ok >> impl_tac >- gvs[avoid_ok_def, SUBSET_DEF] >>
+      strip_tac >> simp[] >> gvs[SUBSET_DEF, avoid_ok_def, allvars_thm]
+      )
+    >- (
+      CCONTR_TAC >> qpat_x_assum `¬MEM x _` mp_tac >> gvs[MAP_EQ_APPEND] >>
+      pairarg_tac >> gvs[MEM_MAP]
+      ) >>
+    gvs[MAP_EQ_APPEND, PULL_EXISTS] >> pairarg_tac >> gvs[EXISTS_PROD] >>
+    rename1 `l1 ++ [(cn,pvs1,ce)] ++ r1` >>
+    last_x_assum mp_tac >> simp[SF DNF_ss] >> strip_tac >> pop_assum kall_tac >>
+    gvs[freshen_mapM_append, freshen_mapM_def] >> rpt (pairarg_tac >> gvs[]) >>
+    first_x_assum drule >> strip_tac >>
+    rename1 `l2 ++ [(cn,pvs2,ce')] ++ r2` >> irule_at Any EQ_REFL >>
+    imp_res_tac fresh_boundvars_LENGTH >> imp_res_tac freshen_mapM_LENGTH >> gvs[] >>
+    simp[MEM_MAP] >>
+    rename1 `freshen_mapM _ _ avoid3 = (_,avoidL)` >>
+    rename1 `fresh_boundvars _ _ _ = (_,avoidB)` >>
+    rename1 `freshen_aux _ _ avoidB = (_,avoidE)` >>
+    qpat_x_assum `freshen_mapM _ _ avoidE = _` kall_tac >>
+    simp[MAP_MAP_o, combinTheory.o_DEF, LAMBDA_PROD] >>
+    irule_at Any freshen_global_mono >> first_x_assum $ irule_at Any >>
+    `EVERY (λ(cn,pvs,ce).
+      set (MAP explode pvs) ⊆ set_of avoid3 ∧ avoid_ok avoid3 ce) l1` by (
+        gvs[EVERY_MEM, FORALL_PROD, SUBSET_DEF, avoid_ok_def] >>
+        metis_tac[]) >>
+    `vars_ok avoidL ∧ set_of avoid3 ⊆ set_of avoidL ∧
+     EVERY (λ(cn,pvs,ce).
+      set (MAP explode pvs) ∪ boundvars (exp_of ce) ⊆ set_of avoidL) l2` by (
+      pop_assum mp_tac >>
+      map_every (fn p => qpat_x_assum p mp_tac)
+        [`freshen_mapM _ _ _ = _`,`vars_ok avoid3`] >>
+      rpt $ pop_assum kall_tac >>
+      map_every qid_spec_tac [`avoid3`,`l2`] >>
+      Induct_on `l1` >> simp[freshen_mapM_def, AND_IMP_INTRO] >>
+      rpt gen_tac >> strip_tac >> rpt (pairarg_tac >> gvs[]) >>
+      drule_all fresh_boundvars_vars >> strip_tac >>
+      drule_all $ cj 1 freshen_aux_mono >> strip_tac >> gvs[] >>
+      last_x_assum $ drule_at $ Pat `freshen_mapM` >> simp[] >> impl_tac
+      >- (gvs[EVERY_MEM, FORALL_PROD, SUBSET_DEF, avoid_ok_def] >> metis_tac[]) >>
+      drule $ cj 1 freshen_aux_avoid_ok >> impl_tac >- gvs[avoid_ok_def, SUBSET_DEF] >>
+      strip_tac >> simp[] >> gvs[SUBSET_DEF, avoid_ok_def, allvars_thm]) >>
+    drule_all fresh_boundvars_rel >> strip_tac >> gvs[] >>
+    rw[]
+    >- gvs[avoid_ok_def, SUBSET_DEF]
+    >- gvs[SUBSET_DEF]
+    >- gvs[avoid_ok_def, SUBSET_DEF, allvars_thm]
+    >- (
+      gvs[BIGUNION_SUBSET, MEM_MAP, PULL_EXISTS, FORALL_PROD, EVERY_MEM] >>
+      gvs[SUBSET_DEF] >> metis_tac[]
+      )
+    >- (gvs[DISJOINT_ALT, SUBSET_DEF] >> metis_tac[])
+    >- (
+      gvs[DISJOINT_ALT, SUBSET_DEF, avoid_ok_def, allvars_thm] >>
+      metis_tac[]
+      )
+    >- (
+      gvs[EVERY_MAP, EVERY_MEM, FORALL_PROD, DISJOINT_ALT,
+          SUBSET_DEF, avoid_ok_def, allvars_thm] >>
+      metis_tac[]
+      )
+    )
+  >- ( (* list case *)
+    rpt (pairarg_tac >> gvs[]) >>
+    rename1 `freshen_aux_list _ ces1 avoid1' = (ces2,_)` >>
+    rename1 `freshen_aux _ ce1' _ = (ce2',_)` >>
+    rename1 `freshen_aux _ ce1 _ = (ce2,_)` >>
+    Cases_on `l1` >> gvs[freshen_aux_def] >>
+    rpt (pairarg_tac >> gvs[]) >>
+    last_x_assum drule_all >> strip_tac >>
+    last_x_assum drule >> strip_tac >>
+    gvs[freshen_aux_list_append, freshen_aux_def] >>
+    rpt (pairarg_tac >> gvs[]) >>
+    first_x_assum $ qspecl_then [`m`,`t`] mp_tac >>
+    simp[] >> impl_tac
+    >- (
+      gvs[EVERY_MEM, avoid_ok_def] >>
+      drule $ cj 1 freshen_aux_mono >> strip_tac >> gvs[] >>
+      gvs[SUBSET_DEF, allvars_thm, contains_var_in_set_of] >> metis_tac[]
+      ) >>
+    strip_tac >> simp[] >> gvs[AC UNION_ASSOC UNION_COMM]
+    )
+QED
+
+Theorem freshen_cexp_freshen_global:
+  ∀ce1 avoid1 ce2 avoid2.
+    freshen_cexp ce1 avoid1 = (ce2,avoid2) ∧
+    avoid_ok avoid1 ce1 ∧
+    NestedCase_free ce1 ∧ letrecs_distinct (exp_of ce1) ∧ cexp_wf ce1
+  ⇒ freshen_global (set_of avoid1) FEMPTY (exp_of ce1) (exp_of ce2)
+Proof
+  rw[freshen_cexp_def] >>
+  irule $ cj 1 freshen_aux_freshen_global >> simp[] >>
+  goal_assum drule >> simp[varmap_rel_def]
+QED
+
+
+
+(****************************** Top-level theorems ******************************)
 
 Definition avoid_set_ok_def:
   avoid_set_ok avoid ce ⇔
@@ -16,16 +1936,48 @@ Definition avoid_set_ok_def:
       ⇒ ∃v. lookup (FST avoid) (implode x) = SOME v
 End
 
+Theorem avoid_set_ok_avoid_ok:
+  avoid_set_ok avoid ce ⇔ avoid_ok avoid ce
+Proof
+  rw[avoid_set_ok_def, avoid_ok_def] >>
+  simp[allvars_thm, SUBSET_DEF] >> eq_tac >> strip_tac >> gvs[] >> gen_tac
+  >- (
+    `∃x'. x = explode x'` by (qexists `implode x` >> simp[]) >>
+    strip_tac >> gvs[] >> res_tac >> simp[GSYM contains_var_in_set_of] >>
+    PairCases_on `avoid` >> simp[contains_var_def] >> fs[]
+    ) >>
+  gvs[SF DNF_ss] >> rw[] >> first_x_assum drule >>
+  `∃x'. x = explode x'` by (qexists `implode x` >> simp[]) >> gvs[] >>
+  simp[GSYM contains_var_in_set_of] >>
+  PairCases_on `avoid` >> gvs[contains_var_def] >> CASE_TAC >> gvs[]
+QED
+
 Theorem freshen_cexp_correctness:
   ∀ce avoid ce' avoid'.
-    freshen_cexp ce avoid = (ce',avoid') ∧
-    avoid_set_ok avoid ce
+    freshen_cexp ce avoid = (ce',avoid') ∧ avoid_set_ok avoid ce ∧
+    NestedCase_free ce ∧ letrecs_distinct (exp_of ce) ∧ cexp_wf ce
   ⇒ exp_of ce ≅ exp_of ce' ∧ avoid_set_ok avoid' ce' ∧ barendregt (exp_of ce') ∧
     (freevars $ exp_of ce' = freevars $ exp_of ce) ∧
-    cns_arities ce' = cns_arities ce ∧
-    (cexp_wf ce ⇒ cexp_wf ce')
+    cns_arities ce' = cns_arities ce ∧ cexp_wf ce' ∧ NestedCase_free ce'
 Proof
-  cheat
+  rpt gen_tac >> strip_tac >> gvs[avoid_set_ok_avoid_ok] >>
+  drule_all freshen_cexp_freshen_global >> strip_tac >>
+  drule freshen_global_freshen_stack >> strip_tac >>
+  dxrule freshen_stack_freshen_subst >> simp[] >>
+  impl_tac >- gvs[avoid_ok_def, allvars_thm] >> strip_tac >>
+  dxrule freshen_subst_exp_alpha >>
+  impl_tac >- gvs[avoid_ok_def] >> strip_tac >>
+  irule_at Any exp_alpha_exp_eq >> simp[] >>
+  drule exp_alpha_freevars >> strip_tac >> simp[] >>
+  gvs[freshen_cexp_def] >>
+  drule_all $ cj 1 freshen_aux_avoid_ok >> strip_tac >> simp[] >>
+  drule_all $ cj 1 freshen_aux_cns_arities >> strip_tac >> simp[] >>
+  drule $ cj 1 freshen_aux_cexp_wf >> impl_tac >- gvs[avoid_ok_def] >> strip_tac >>
+  drule $ cj 1 freshen_aux_NestedCase_free >> rw[] >>
+  simp[barendregt_def] >>
+  irule_at Any freshen_global_unique_boundvars >> goal_assum drule >> simp[] >>
+  irule DISJOINT_SUBSET >> irule_at Any freshen_global_boundvars >>
+  goal_assum drule >> gvs[avoid_ok_def, allvars_thm]
 QED
 
 Theorem avoid_set_ok_boundvars_of:
@@ -33,5 +1985,7 @@ Theorem avoid_set_ok_boundvars_of:
 Proof
   cheat
 QED
+
+(**********)
 
 val _ = export_theory();
